Prove exceptionless determinism and its helpers

src/Core_Erlang_Side_Effects.v
@@ -4,6 +4,7 @@ Require Core_Erlang_Environment.
 Module Side_Effects.
 
 Export Core_Erlang_Syntax.Syntax.
+Export Core_Erlang_Helpers.Helpers.
 
 Import ListNotations.
 
@@ -24,15 +25,35 @@ Compute concatn [(Input, [VLit (Atom "a"%string)] )]
                   [(Input, [VLit (Atom "c"%string)] )] ] 
                 0. *)
 
-Definition nth_def {A : Type} (l : list A) (def : A) (i : nat) :=
+Definition nth_def {A : Type} (l : list A) (def err : A) (i : nat) :=
 match i with
 | 0 => def
-| S i' => nth i' l def
+| S i' => nth i' l err
 end.
 
-Compute nth_def [4; 7; 8] 3 2 = 7.
+Compute nth_def [4; 7; 8] 3 0 2 = 7.
 Compute nth_def [ [(Input, [VLit (Atom "a"%string)] )];
                   [(Input, [VLit (Atom "a"%string)] ); (Input, [VLit (Atom "b"%string)] )]; 
-                  [(Input, [VLit (Atom "a"%string)] ); (Input, [VLit (Atom "b"%string)] ); (Input, [VLit (Atom "c"%string)] )]] [] 2 = [(Input, [VLit (Atom "a"%string)] ); (Input, [VLit (Atom "b"%string)] )].
+                  [(Input, [VLit (Atom "a"%string)] ); (Input, [VLit (Atom "b"%string)] ); (Input, [VLit (Atom "c"%string)] )]] [] [] 2 = [(Input, [VLit (Atom "a"%string)] ); (Input, [VLit (Atom "b"%string)] )].
+
+Import Omega.
+
+Lemma nth_def_eq {A : Type} (l : list A) (i : nat) (e1 def err : A):
+  nth_def (e1::l) def err (S i) = nth_def l e1 err i.
+Proof.
+  simpl. destruct i.
+  * simpl. reflexivity.
+  * simpl. reflexivity.
+Qed.
+
+Theorem last_nth_equal {A : Type} (l : list A) (def err : A) :
+  last l def = nth_def l def err (length l).
+Proof.
+  induction l.
+  * auto.
+  * simpl. rewrite IHl. destruct l.
+    - auto.
+    - simpl. auto.
+Qed.
 
 End Side_Effects.
