src/Core_Erlang_Determinism_Helpers.v
@@ -1,72 +1,69 @@
-Require Core_Erlang_Semantics.
+Require Core_Erlang_Tactics.
 
 From Coq Require Import Arith.PeanoNat.
 
 (** Helper lemmas for determinism *)
 Module Determinism_Helpers.
 
-Export Core_Erlang_Environment.Environment.
+Export Core_Erlang_Semantics.Semantics.
+Import Core_Erlang_Tactics.Tactics.
 
 Import ListNotations.
-(* Export Coq.Init.Logic. *)
 
-Section List_Length_Theorems.
-
-Proposition list_length {A : Type} {a : A} {l : list A} : length (a :: l) > 0.
-Proof.
-  simpl. apply Nat.lt_0_succ.
-Qed.
-
-Theorem last_element_equal {A : Type} (l : list A) (def def2 : A):
-  last l def = last (def :: l) def2.
-Proof.
-  induction l.
-  * auto.
-  * simpl. rewrite IHl. simpl. destruct l; auto.
-Qed.
-
-Theorem last_nth_equal (l : list nat) (def : nat) :
-  last l def = nth_id l def (length l).
-Proof.
-  induction l.
-  * auto.
-  * simpl. rewrite IHl. destruct l.
-    - auto.
-    - simpl. auto.
-Qed.
-
-End List_Length_Theorems.
-
-Lemma concatn_app {eff1 x1 : SideEffectList} {x6 : list SideEffectList} {i : nat} : 
+(* Lemma concatn_app {eff1 x1 : SideEffectList} {x6 : list SideEffectList} {i : nat} : 
   concatn eff1 (x1 :: x6) (S i) = concatn (eff1 ++ x1) x6 i.
 Proof.
   induction i.
   * simpl_concatn. reflexivity.
   * simpl_concatn. simpl_concatn_H IHi. reflexivity.
 Qed.
-
+ *)
 (** Attibute restriction to a smaller list *)
 Lemma restrict_helper {env : Environment} {eff1 : SideEffectList} {exps : list Expression} 
     (a : Expression) (x1 : SideEffectList) (x6 : list SideEffectList) (x0 : Value) 
     (x3 : list Value) (id' : nat) (ids : list nat) (id : nat):
 (forall i : nat,
     i < Datatypes.length (a :: exps) ->
-    | env, nth_id (id'::ids) id i, nth i (a :: exps) ErrorExp, concatn eff1 (x1 :: x6) i | -e>
-    | nth_id (id'::ids) id (S i), inl (nth i (x0 :: x3) ErrorValue), concatn eff1 (x1 :: x6) (S i) |)
+    | env, nth_def (id'::ids) id 0 i, nth i (a :: exps) ErrorExp, nth_def (x1 :: x6) eff1 [] i | -e>
+    | nth_def (id'::ids) id 0 (S i), inl (nth i (x0 :: x3) ErrorValue), nth_def (x1 :: x6) eff1 [] (S i) |)
 ->
 forall i : nat,
     i < Datatypes.length exps ->
-    | env, nth_id ids id' i, nth i exps ErrorExp, concatn (eff1 ++ x1) x6 i | -e>
-    | nth_id ids id' (S i), inl (nth i x3 ErrorValue), concatn (eff1 ++ x1) x6 (S i) |
+    | env, nth_def ids id' 0 i, nth i exps ErrorExp, nth_def x6 x1 [] i | -e>
+    | nth_def ids id' 0 (S i), inl (nth i x3 ErrorValue), nth_def x6 x1 [] (S i) |
 .
 Proof.
   intros.
   assert (S i < Datatypes.length (a :: exps)) as A1.
   { simpl. apply lt_n_S. assumption. } pose (E := H (S i) A1). 
-  pose (P1 := @concatn_app eff1 x1 x6 i).
+  (* pose (P1 := @concatn_app eff1 x1 x6 i).
   pose (P2 := @concatn_app eff1 x1 x6 (S i)).
-  rewrite P1, P2 in E. simpl in E. simpl. unfold nth_id. exact E.
+  rewrite P1, P2 in E. *) simpl in E. simpl. unfold nth_def. exact E.
 Qed.
+
+Ltac empty_list_in_hypo :=
+match goal with
+| [H : 0 = length _ |- _ ] => apply eq_sym, length_zero_iff_nil in H
+| [H : length _ = 0 |- _ ] => apply length_zero_iff_nil in H
+| _ => idtac
+end.
+
+Ltac single_unfold_list :=
+match goal with
+| [ Hyp : Datatypes.length ?l = 0 |- _] => apply length_zero_iff_nil in Hyp; subst
+| [ Hyp : 0 = Datatypes.length ?l |- _] => apply eq_sym, length_zero_iff_nil in Hyp; subst
+| [ Hyp : Datatypes.length ?l = S ?n |- _] => symmetry in Hyp; single_unfold_list
+| [ Hyp : S ?n = Datatypes.length ?l |- _] => 
+   pose (element_exist _ _ Hyp);
+   match goal with
+   | [H' : exists x l', _ = x::l' |- _] => 
+     inversion H';
+     match goal with
+     | [H'' : exists l', _ = ?x::l' |- _] => inversion H''; subst; simpl in Hyp; inversion Hyp
+     end
+   end
+end
+.
 
 (** Value lists are equal ased on the determinism hypotheses *)
 Lemma list_equality {env : Environment} {exps : list Expression} {eff1 : SideEffectList} : 
@@ -74,23 +71,23 @@ forall vals vals0 : list Value, forall eff eff4 : list SideEffectList,
 forall id ids ids0,
   (forall i : nat,
      i < Datatypes.length exps ->
-     | env, nth_id ids id i, nth i exps ErrorExp, concatn eff1 eff i | 
+     | env, nth_def ids id 0 i, nth i exps ErrorExp, nth_def eff eff1 [] i | 
      -e> 
-     | nth_id ids id (S i), inl (nth i vals ErrorValue), concatn eff1 eff (S i) |)
+     | nth_def ids id 0 (S i), inl (nth i vals ErrorValue), nth_def eff eff1 [] (S i) |)
 ->
 (forall i : nat,
      i < Datatypes.length exps ->
      forall (v2 : Value + Exception) (eff'' : SideEffectList) (id'' : nat),
-     | env, nth_id ids id i, nth i exps ErrorExp, concatn eff1 eff i |
+     | env, nth_def ids id 0 i, nth i exps ErrorExp, nth_def eff eff1 [] i |
      -e>
      | id'', v2, eff'' | ->
-     inl (nth i vals ErrorValue) = v2 /\ concatn eff1 eff (S i) = eff'' /\ nth_id ids id (S i) = id'')
+     inl (nth i vals ErrorValue) = v2 /\ nth_def eff eff1 [] (S i) = eff'' /\ nth_def ids id 0 (S i) = id'')
 ->
 (forall i : nat,
      i < Datatypes.length exps ->
-     | env, nth_id ids0 id i, nth i exps ErrorExp, concatn eff1 eff4 i |
+     | env, nth_def ids0 id 0 i, nth i exps ErrorExp, nth_def eff4 eff1 [] i |
      -e> 
-     | nth_id ids0 id (S i), inl (nth i vals0 ErrorValue), concatn eff1 eff4 (S i) |)
+     | nth_def ids0 id 0 (S i), inl (nth i vals0 ErrorValue), nth_def eff4 eff1 [] (S i) |)
 ->
 Datatypes.length exps = Datatypes.length vals0
 ->
@@ -107,19 +104,18 @@ length exps = length ids0
 eff = eff4 /\ vals = vals0 /\ ids = ids0.
 Proof.
   generalize dependent eff1. induction exps.
-  * intros. inversion H3. inversion H2. inversion H4. inversion H5. inversion H6. inversion H7.
-    repeat (unfold_list).
-    auto.
+  * intros. simpl in H3, H2, H4, H5, H6, H7.
+    repeat (empty_list_in_hypo).
+    subst. auto.
   * intros. inversion H3. inversion H2. inversion H4. inversion H5. inversion H6. inversion H7.
   
   (* first elements are the same *)
     single_unfold_list. single_unfold_list.
     single_unfold_list. single_unfold_list.
     single_unfold_list. single_unfold_list.
-    pose (P1 := H1 0 list_length). simpl_concatn_H P1.
-    pose (P2 := H0 0 list_length (inl x7) (concatn eff1 (x9 :: x10) 1) x).
-    simpl_concatn_H P2.
-    pose (P3 := P2 P1). inversion P3. inversion H25. inversion H27. apply app_inv_head in H28.
+    pose (P1 := H1 0 list_length).
+    pose (P2 := H0 0 list_length (inl x7) (nth_def (x9 :: x10) eff1 [] 1) x).
+    pose (P3 := P2 P1). inversion P3. inversion H25. inversion H27. simpl in H28. simpl in H30.
     subst.
   (* remaining lists are the same *)
 
@@ -128,9 +124,9 @@ Proof.
     assert (
       (forall i : nat,
     i < Datatypes.length exps ->
-    | env, nth_id x2 x i, nth i exps ErrorExp, concatn (eff1 ++ x9) x4 i | -e> 
-    | nth_id x2 x (S i), inl (nth i x6 ErrorValue),
-    concatn (eff1 ++ x9) x4 (S i) |)
+    | env, nth_def x2 x 0 i, nth i exps ErrorExp, nth_def x4 x9 [] i | -e> 
+    | nth_def x2 x 0 (S i), inl (nth i x6 ErrorValue),
+    nth_def x4 x9 [] (S i) |)
     ).
     {
       intros. pose (P4 := restrict_helper a _ _ _ _ _ _ _ H i H28). assumption.
@@ -139,35 +135,28 @@ Proof.
       (forall i : nat,
       i < Datatypes.length exps ->
       forall (v2 : Value + Exception) (eff'' : SideEffectList) (id'' : nat),
-      | env, nth_id x2 x i, nth i exps ErrorExp, concatn (eff1 ++ x9) x4 i | -e> | id'', v2, eff'' | ->
-      inl (nth i x6 ErrorValue) = v2 /\ concatn (eff1 ++ x9) x4 (S i) = eff'' /\ nth_id x2 x (S i) = id'')
+      | env, nth_def x2 x 0 i, nth i exps ErrorExp, nth_def x4 x9 [] i | -e> | id'', v2, eff'' | ->
+      inl (nth i x6 ErrorValue) = v2 /\ nth_def x4 x9 [] (S i) = eff'' /\ nth_def x2 x 0 (S i) = id'')
     ).
     {
       intros. assert (S i < Datatypes.length (a::exps)). { simpl. omega. } 
-      pose (P4 := H0 (S i) H31 v2 eff'' id''). simpl nth in P4. rewrite concatn_app in P4. 
-      rewrite concatn_app in P4. exact (P4 H30).
+      pose (P4 := H0 (S i) H31 v2 eff'' id''). simpl nth in P4. exact (P4 H30).
     }
     assert (
      (forall i : nat,
     i < Datatypes.length exps ->
-    | env, nth_id x0 x i, nth i exps ErrorExp, concatn (eff1 ++ x9) x10 i | -e>
-    | nth_id x0 x (S i), inl (nth i x8 ErrorValue),
-    concatn (eff1 ++ x9) x10 (S i) |)
+    | env, nth_def x0 x 0 i, nth i exps ErrorExp, nth_def x10 x9 [] i | -e>
+    | nth_def x0 x 0 (S i), inl (nth i x8 ErrorValue),
+    nth_def x10 x9 [] (S i) |)
     ).
     {
       intros. assert (S i < Datatypes.length (a :: exps)). { simpl. omega. } 
-      pose (P4 := H1 (S i) H31). simpl nth in P4. rewrite concatn_app in P4. 
-      rewrite concatn_app in P4. simpl in P4. assumption.
+      pose (P4 := H1 (S i) H31). simpl nth in P4. assumption.
     }
     (* simpl list lengths *)
     inversion H10. inversion H11. inversion H12. inversion H13. inversion H14.
-    pose (IH := IHexps (eff1 ++ x9) x6 x8 x4 x10 x x2 x0 H28 H29 H30 H32 H26 H33 H34 H35 H36). 
+    pose (IH := IHexps x9 x6 x8 x4 x10 x x2 x0 H28 H29 H30 H32 H26 H33 H34 H35 H36). 
     inversion IH. inversion H37. subst. auto.
-Qed.
-
-Proposition nat_ge_or : forall {n m : nat}, n >= m <-> n = m \/ n > m.
-Proof.
-  intros. omega.
 Qed.
 
 (** Based on determinism hypotheses, the same clause was chosen in case evaluation *)
@@ -228,18 +217,18 @@ length ids0 = length vals0
 (forall i : nat,
      i < Datatypes.length exps ->
      forall (v2 : Value + Exception) (eff'' : SideEffectList) (id'' : nat),
-     | env, nth_id ids id i, nth i exps ErrorExp, concatn eff1 eff i | -e> | id'', v2, eff'' | ->
-     inl (nth i vals ErrorValue) = v2 /\ concatn eff1 eff (S i) = eff'' /\ nth_id ids id (S i) = id'')
+     | env, nth_def ids id 0 i, nth i exps ErrorExp, nth_def eff eff1 [] i | -e> | id'', v2, eff'' | ->
+     inl (nth i vals ErrorValue) = v2 /\ nth_def eff eff1 [] (S i) = eff'' /\ nth_def ids id 0 (S i) = id'')
 ->
 (forall j : nat,
      j < Datatypes.length vals0 ->
-     | env, nth_id ids0 id j, nth j exps ErrorExp, concatn eff1 eff5 j | -e>
-     | nth_id ids0 id (S j), inl (nth j vals0 ErrorValue),
-     concatn eff1 eff5 (S j) |)
+     | env, nth_def ids0 id 0 j, nth j exps ErrorExp, nth_def eff5 eff1 [] j | -e>
+     | nth_def ids0 id 0 (S j), inl (nth j vals0 ErrorValue),
+     nth_def eff5 eff1 [] (S j) |)
 ->
 | env, last ids0 id, nth (Datatypes.length vals0) exps ErrorExp,
-      concatn eff1 eff5 (Datatypes.length vals0) | -e> | id'', inr ex,
-      concatn eff1 eff5 (Datatypes.length vals0) ++ eff3 |
+      last eff5 eff1 | -e> | id'', inr ex,
+      eff3 |
 ->
 False.
 Proof.
@@ -261,32 +250,30 @@ Proof.
       assert (Datatypes.length exps = S (Datatypes.length eff)) as Helper. { auto. }
       assert (Datatypes.length ids0 = Datatypes.length vals0) as Helper2. { auto. }
       assert (Datatypes.length exps = Datatypes.length ids) as Helper3. { auto. }
-      pose (EE1 := element_exist _ _ _ (eq_sym H10)).
-      pose (EE2 := element_exist _ _ _ H1).
+      pose (EE1 := element_exist _ _ (eq_sym H10)).
+      pose (EE2 := element_exist _ _ H1).
       rewrite H in H0.
-      pose (EE3 := element_exist _ _ _ (eq_sym H0)).
+      pose (EE3 := element_exist _ _ (eq_sym H0)).
       rewrite <- H1 in H4. rewrite H10 in H3.
-      pose (EE4 := element_exist _ _ _ H3).
-      pose (EE5 := element_exist _ _ _ (eq_sym H4)).
+      pose (EE4 := element_exist _ _ H3).
+      pose (EE5 := element_exist _ _ (eq_sym H4)).
       inversion EE1 as [e]. inversion EE2 as [v]. inversion EE3 as [v'].
       inversion EE4 as [id0']. inversion EE5 as [id0'']. 
       inversion H13. inversion H14. inversion H15. inversion H16. inversion H17. subst.
-      pose (P0 := H6 0 H11). simpl_concatn_H P0.
-      pose (P1 := H5 0 H8 (inl v) (eff1 ++ s ++ [])). simpl_concatn_H P1.
-      pose (P2 := P1 _ P0). destruct P2. destruct H18, H19. apply app_inv_head in H18. subst.
+      pose (P0 := H6 0 H11).
+      pose (P1 := H5 0 H8 (inl v) (s)).
+      pose (P2 := P1 _ P0). destruct P2. destruct H18, H19. simpl in H18, H19. subst.
     (* other elements *)
       inversion H1.
-      eapply IHeff with (exps := x) (vals := x1) (vals0 := x0) (eff1 := eff1 ++ s)
+      eapply IHeff with (exps := x) (vals := x1) (vals0 := x0) (eff1 := s)
                       (ids := x2) (ids0 := x3) (id := id0'') (eff5 := eff5); auto.
         + intuition.
         + intros. assert (S i < Datatypes.length (e :: x)). { simpl. omega. }
-          pose (A := H5 (S i) H21 v2 eff''). rewrite concatn_app, concatn_app in A.
-          simpl in A, H20.
+          pose (A := H5 (S i) H21 v2 eff''). simpl in A, H20.
           pose (B := A _ H20). assumption.
         + intros. assert (S j < Datatypes.length (v :: x0)). { omega. } 
-          pose (A := H6 (S j) H20). 
-          rewrite concatn_app, concatn_app in A. simpl in A. exact A.
-        + rewrite <- last_element_equal in H7. simpl in H7. rewrite concatn_app in H7. exact H7.
+          pose (A := H6 (S j) H20). exact A.
+        + rewrite <- last_element_equal, <- last_element_equal in H7. exact H7.
 Qed.
 
 (** Side effect equality until the ith element using concatn *)
@@ -307,22 +294,21 @@ length ids0 = length vals0
 (forall i : nat,
      i < Datatypes.length exps ->
      forall (v2 : Value + Exception) (eff'' : SideEffectList) (id'' : nat),
-     | env, nth_id ids id i, nth i exps ErrorExp, concatn eff1 eff i | -e> | id'', v2, eff'' | ->
-     inl (nth i vals ErrorValue) = v2 /\ concatn eff1 eff (S i) = eff'' /\ nth_id ids id (S i) = id'')
+     | env, nth_def ids id 0 i, nth i exps ErrorExp, nth_def eff eff1 [] i | -e> | id'', v2, eff'' | ->
+     inl (nth i vals ErrorValue) = v2 /\ nth_def eff eff1 [] (S i) = eff'' /\ nth_def ids id 0 (S i) = id'')
 ->
 (forall j : nat,
      j < Datatypes.length vals0 ->
-     | env, nth_id ids0 id j, nth j exps ErrorExp, concatn eff1 eff5 j | -e>
-     | nth_id ids0 id (S j), inl (nth j vals0 ErrorValue),
-     concatn eff1 eff5 (S j) |)
+     | env, nth_def ids0 id 0 j, nth j exps ErrorExp, nth_def eff5 eff1 [] j | -e>
+     | nth_def ids0 id 0 (S j), inl (nth j vals0 ErrorValue),
+     nth_def eff5 eff1 [] (S j) |)
 ->
 | env, last ids0 id, nth (Datatypes.length vals0) exps ErrorExp,
-      concatn eff1 eff5 (Datatypes.length vals0) | -e> | id'', inr ex,
-      concatn eff1 eff5 (Datatypes.length vals0) ++ eff3 |
+      last eff5 eff1 | -e> | id'', inr ex, eff3 |
 ->
   False.
 Proof.
-  intros. simpl_concatn. pose (P := firstn_eq eff5 exps vals vals0 _ _ _ _ _ _ _
+  intros. pose (P := firstn_eq eff5 exps vals vals0 _ _ _ _ _ _ _
                                 H H0 H1 H2 H3 H4 H5 H6 H7). inversion P.
 Qed.
 
@@ -334,18 +320,18 @@ Lemma firstn_eq_rev {env : Environment} {eff : list SideEffectList} :
 (forall j : nat,
      j < Datatypes.length vals ->
      forall (v2 : Value + Exception) (eff'' : SideEffectList) (id'' : nat),
-     | env, nth_id ids id j, nth j exps ErrorExp, concatn eff1 eff j | -e> | id'', v2, eff'' | ->
-     inl (nth j vals ErrorValue) = v2 /\ concatn eff1 eff (S j) = eff'' /\ nth_id ids id (S j) = id'')
+     | env, nth_def ids id 0 j, nth j exps ErrorExp, nth_def eff eff1 [] j | -e> | id'', v2, eff'' | ->
+     inl (nth j vals ErrorValue) = v2 /\ nth_def eff eff1 [] (S j) = eff'' /\ nth_def ids id 0 (S j) = id'')
 ->
 (forall i : nat,
      i < Datatypes.length exps ->
-     | env, nth_id ids0 id i, nth i exps ErrorExp, concatn eff1 eff5 i | -e>
-     | nth_id ids0 id (S i), inl (nth i vals0 ErrorValue),
-     concatn eff1 eff5 (S i) |) ->
+     | env, nth_def ids0 id 0 i, nth i exps ErrorExp, nth_def eff5 eff1 [] i | -e>
+     | nth_def ids0 id 0 (S i), inl (nth i vals0 ErrorValue),
+     nth_def eff5 eff1 [] (S i) |) ->
 (forall (v2 : Value + Exception) (eff'' : SideEffectList) (id'' : nat),
         | env, last ids id, nth (Datatypes.length vals) exps ErrorExp,
-        concatn eff1 eff (Datatypes.length vals) | -e> | id'', v2, eff'' | ->
-        inr ex = v2 /\ concatn eff1 eff (Datatypes.length vals) ++ eff2 = eff'' /\ id' = id'')
+        last eff eff1 | -e> | id'', v2, eff'' | ->
+        inr ex = v2 /\ eff2 = eff'' /\ id' = id'')
 ->
 Datatypes.length vals < Datatypes.length exps ->
 Datatypes.length eff = Datatypes.length vals ->
@@ -371,31 +357,30 @@ Proof.
       assert (S (Datatypes.length eff) = Datatypes.length vals) as Helper1. { auto. }
       assert (Datatypes.length exps = Datatypes.length ids0) as Helper2. { auto. }
       (* single_unfold_list H9. *)
-      pose (EE1 := element_exist Expression (length eff5) exps (eq_sym H5)).
-      pose (EE2 := element_exist Value (length eff) vals H9).
+      pose (EE1 := element_exist (length eff5) exps (eq_sym H5)).
+      pose (EE2 := element_exist (length eff) vals H9).
       rewrite H5 in H4, H6. rewrite <- H9 in H7.
-      pose (EE3 := element_exist Value (length eff5) vals0 H4).
-      pose (EE4 := element_exist _ _ _ (eq_sym H7)).
-      pose (EE5 := element_exist _ _ _ H6).
-
+      pose (EE3 := element_exist (length eff5) vals0 H4).
+      pose (EE4 := element_exist _ _ (eq_sym H7)).
+      pose (EE5 := element_exist _ _ H6).
+      
       inversion EE1 as [e]. inversion EE2 as [v]. inversion EE3 as [v'].
       inversion EE4 as [id0']. inversion EE5 as [id0'']. 
       inversion H13. inversion H14. inversion H15. inversion H16. inversion H17. subst.
-      pose (P0 := H0 0 H8). simpl_concatn_H P0.
-      pose (P1 := H 0 H11 (inl v') (eff1 ++ s ++ [])). simpl_concatn_H P1.
-      pose (P2 := P1 _ P0). destruct P2. destruct H19. apply app_inv_head in H19. inversion H18. subst.
+      pose (P0 := H0 0 H8).
+      pose (P1 := H 0 H11 (inl v') s).
+      pose (P2 := P1 _ P0). destruct P2. destruct H19. inversion H18. simpl in H19, H20. subst.
     (* other elements *)
       inversion H3.
-      apply IHeff with (exps := x) (vals := x0) (eff1 := eff1 ++ s) (vals0 := x1)
+      apply IHeff with (exps := x) (vals := x0) (eff1 := s) (vals0 := x1)
                   (ids := x2) (ids0 := x3) (id := id0'') (ex := ex) (eff5 := eff5)
                   (eff2 := eff2) (id' := id'); auto.
         + intros. assert (S j < Datatypes.length (v' :: x0)). { simpl. omega. } 
-          pose (A := H (S j) H22 v2 eff''). rewrite concatn_app, concatn_app in A. simpl in A. 
+          pose (A := H (S j) H22 v2 eff'').
           pose (B := A _ H21). assumption.
         + intros. assert (S i < Datatypes.length (e :: x)). { simpl. omega. } 
-          pose (A := H0 (S i) H21). rewrite concatn_app, concatn_app in A. simpl in A. exact A.
-        + intros. rewrite <- last_element_equal in H1. simpl in H1. rewrite concatn_app in H1.
-          apply H1. assumption.
+          pose (A := H0 (S i) H21). exact A.
+        + intros. rewrite <- last_element_equal, <- last_element_equal in H1. apply H1. assumption.
         + intuition.
         + inversion H7. omega.
 Qed.
@@ -408,18 +393,18 @@ Lemma eff_until_i_rev {env : Environment} {eff : list SideEffectList} :
 (forall j : nat,
      j < Datatypes.length vals ->
      forall (v2 : Value + Exception) (eff'' : SideEffectList) (id'' : nat),
-     | env, nth_id ids id j, nth j exps ErrorExp, concatn eff1 eff j | -e> | id'', v2, eff'' | ->
-     inl (nth j vals ErrorValue) = v2 /\ concatn eff1 eff (S j) = eff'' /\ nth_id ids id (S j) = id'')
+     | env, nth_def ids id 0 j, nth j exps ErrorExp, nth_def eff eff1 [] j | -e> | id'', v2, eff'' | ->
+     inl (nth j vals ErrorValue) = v2 /\ nth_def eff eff1 [] (S j) = eff'' /\ nth_def ids id 0 (S j) = id'')
 ->
 (forall i : nat,
      i < Datatypes.length exps ->
-     | env, nth_id ids0 id i, nth i exps ErrorExp, concatn eff1 eff5 i | -e>
-     | nth_id ids0 id (S i), inl (nth i vals0 ErrorValue),
-     concatn eff1 eff5 (S i) |) ->
+     | env, nth_def ids0 id 0 i, nth i exps ErrorExp, nth_def eff5 eff1 [] i | -e>
+     | nth_def ids0 id 0 (S i), inl (nth i vals0 ErrorValue),
+     nth_def eff5 eff1 [] (S i) |) ->
 (forall (v2 : Value + Exception) (eff'' : SideEffectList) (id'' : nat),
         | env, last ids id, nth (Datatypes.length vals) exps ErrorExp,
-        concatn eff1 eff (Datatypes.length vals) | -e> | id'', v2, eff'' | ->
-        inr ex = v2 /\ concatn eff1 eff (Datatypes.length vals) ++ eff2 = eff'' /\ id' = id'')
+        last eff eff1 | -e> | id'', v2, eff'' | ->
+        inr ex = v2 /\ eff2 = eff'' /\ id' = id'')
 ->
 Datatypes.length vals < Datatypes.length exps ->
 Datatypes.length eff = Datatypes.length vals ->
@@ -430,15 +415,8 @@ length ids = length vals
 ->
 False.
 Proof.
-  intros. simpl_concatn. apply (firstn_eq_rev eff5 exps vals vals0 eff1 _ _ _ _ _ _
+  intros. apply (firstn_eq_rev eff5 exps vals vals0 eff1 _ _ _ _ _ _
                                    H H0 H1 H2 H3 H4 H5 H6 H7).
-Qed.
-
-Lemma nat_exist {n m : nat} : n < m -> exists x, m = S x.
-Proof.
-  intros. inversion H.
-  * apply ex_intro with n. reflexivity.
-  * apply ex_intro with m0. reflexivity.
 Qed.
 
 (** First i element are equal with concatn *)
@@ -447,17 +425,17 @@ Lemma con_n_equality {env : Environment} {eff : list SideEffectList} :
 (forall j : nat,
     j < i ->
     forall (v2 : Value + Exception) (eff'' : SideEffectList) (id'' : nat),
-    | env, nth_id ids id j, nth j exps ErrorExp, concatn eff1 eff j | -e> | id'', v2, eff'' | ->
-    inl (nth j vals ErrorValue) = v2 /\ concatn eff1 eff (S j) = eff'' /\ nth_id ids id (S j) = id'')
+    | env, nth_def ids id 0 j, nth j exps ErrorExp, nth_def eff eff1 [] j | -e> | id'', v2, eff'' | ->
+    inl (nth j vals ErrorValue) = v2 /\ nth_def eff eff1 [] (S j) = eff'' /\ nth_def ids id 0 (S j) = id'')
 ->
 (forall j : nat,
      j < i0 ->
-     | env, nth_id ids0 id j, nth j exps ErrorExp, concatn eff1 eff6 j | -e>
-     | nth_id ids0 id (S j), inl (nth j vals0 ErrorValue),
-     concatn eff1 eff6 (S j) |)
+     | env, nth_def ids0 id 0 j, nth j exps ErrorExp, nth_def eff6 eff1 [] j | -e>
+     | nth_def ids0 id 0 (S j), inl (nth j vals0 ErrorValue),
+     nth_def eff6 eff1 [] (S j) |)
 ->
 (forall (v2 : Value + Exception) (eff'' : SideEffectList) (id'' : nat),
-     | env, last ids id, nth i exps ErrorExp, concatn eff1 eff i | -e> | id'', v2, eff'' | ->
+     | env, last ids id, nth i exps ErrorExp, last eff eff1 | -e> | id'', v2, eff'' | ->
      inr ex = v2 /\ eff3 = eff'' /\ id' = id'')
 ->
 Datatypes.length eff = i ->
@@ -477,18 +455,18 @@ Proof.
     simpl in H8, P. apply length_zero_iff_nil in H8. subst.
     pose (P2 := H1 _ _ _ P). inversion P2. congruence.
   * intros. inversion H2. simpl in H2. rewrite <- H2 in H4.
-    pose (EE1 := element_exist Value (length eff) vals (eq_sym H4)). 
+    pose (EE1 := element_exist (length eff) vals (eq_sym H4)). 
     inversion EE1 as [v]. inversion H12 as [vs]. destruct eff6.
     - simpl in H7. subst. rewrite <- H7 in H10. inversion H10.
     - subst. simpl. (* simpl_concatn_H IHeff. rewrite concatn_app, concatn_app. simpl_concatn. *)
       simpl in H7. (* single_unfold_list H6. *) 
-      pose (EE2 := element_exist Value (length eff6) vals0 H7). inversion EE2. 
+      pose (EE2 := element_exist (length eff6) vals0 H7). inversion EE2. 
       inversion H2.
-      pose (NE := nat_exist H3). inversion NE.
-      pose (EE3 := element_exist Expression x1 exps (eq_sym H13)). inversion EE3. inversion H14.
+      pose (NE := nat_lt_zero _ _  H3). inversion NE.
+      pose (EE3 := element_exist x1 exps (eq_sym H13)). inversion EE3. inversion H14.
       subst. 
-      pose (EE4 := element_exist _ _ _ (eq_sym H8)).
-      pose (EE5 := element_exist _ _ _ (eq_sym H9)).
+      pose (EE4 := element_exist _ _ (eq_sym H8)).
+      pose (EE5 := element_exist _ _ (eq_sym H9)).
       inversion EE4 as [id0']. inversion EE5 as [id0''].
       inversion H5. inversion H15. subst.
       assert (s = a /\ id0' = id0''). {
@@ -496,21 +474,20 @@ Proof.
         assert (0 < Datatypes.length (x :: x0)). {  simpl. omega. }
         pose (P := H0 0 H16).
         assert (0 < S (Datatypes.length eff)). {  simpl. omega. }
-        pose (P2 := H 0 H17 (inl (nth 0 (x :: x0) ErrorValue)) (concatn eff1 (s :: eff6) 1) _ P). 
+        pose (P2 := H 0 H17 (inl (nth 0 (x :: x0) ErrorValue)) (nth_def (s :: eff6) eff1 [] 1) _ P). 
         inversion P2.
-        simpl_concatn_H H19. destruct H19. apply app_inv_head in H19. auto.
+        destruct H19. auto.
       }
       destruct H16. subst.
       
-      eapply IHeff with (exps := x3) (vals := vs) (vals0 := x0) (eff1 := eff1 ++ a)
+      eapply IHeff with (exps := x3) (vals := vs) (vals0 := x0) (eff1 := a)
                         (i0 := length x0) (ids := x4) (ids0 := x5); auto.
       + intros. assert (S j < S (Datatypes.length eff)). { simpl. omega. }
-        pose (P := H (S j) H18 v2 eff'' id''). 
-        rewrite concatn_app, concatn_app in P. pose (P H17). assumption.
+        pose (P := H (S j) H18 v2 eff'' id''). pose (P H17). assumption.
       + intros. assert (S j < Datatypes.length (x :: x0)). { simpl. omega. }
-        pose (P := H0 (S j) H17). rewrite concatn_app, concatn_app in P. simpl in P. exact P.
-      + intros. apply H1. rewrite concatn_app.
-        rewrite (last_element_equal _ _ id) in H16.
+        pose (P := H0 (S j) H17). exact P.
+      + intros. apply H1.
+        rewrite (last_element_equal _ _ id), (last_element_equal _ _ eff1) in H16.
         exact H16.
       + intuition.
       + intuition.
@@ -525,14 +502,14 @@ Lemma list_equal_until_i {env : Environment} {eff : list SideEffectList} :
 (forall j : nat,
     j < Datatypes.length vals ->
     forall (v2 : Value + Exception) (eff'' : SideEffectList) (id'' : nat),
-    | env, nth_id ids id j, nth j exps ErrorExp, concatn eff1 eff j | -e> | id'', v2, eff'' | ->
-    inl (nth j vals ErrorValue) = v2 /\ concatn eff1 eff (S j) = eff'' /\ nth_id ids id (S j) = id'')
+    | env, nth_def ids id 0 j, nth j exps ErrorExp, nth_def eff eff1 [] j | -e> | id'', v2, eff'' | ->
+    inl (nth j vals ErrorValue) = v2 /\ nth_def eff eff1 [] (S j) = eff'' /\ nth_def ids id 0 (S j) = id'')
 ->
 (forall j : nat,
      j < Datatypes.length vals0 ->
-     | env, nth_id ids0 id j, nth j exps ErrorExp, concatn eff1 eff6 j | -e> 
-     | nth_id ids0 id (S j), inl (nth j vals0 ErrorValue),
-     concatn eff1 eff6 (S j) |)
+     | env, nth_def ids0 id 0 j, nth j exps ErrorExp, nth_def eff6 eff1 [] j | -e> 
+     | nth_def ids0 id 0 (S j), inl (nth j vals0 ErrorValue),
+     nth_def eff6 eff1 [] (S j) |)
 ->
 Datatypes.length vals = Datatypes.length vals0
 ->
@@ -552,32 +529,31 @@ Proof.
   * intros. inversion H2. apply eq_sym, length_zero_iff_nil in H8. subst. simpl in H1. 
     apply eq_sym, length_zero_iff_nil in H1. subst. simpl in H3. apply length_zero_iff_nil in H3. 
     apply length_zero_iff_nil in H5. apply length_zero_iff_nil in H6. subst. auto.
-  * intros. simpl in H2. rewrite <- H2 in H1. rewrite <- H1 in H3. pose (NE := nat_exist H4). inversion NE.
+  * intros. simpl in H2. rewrite <- H2 in H1. rewrite <- H1 in H3. pose (NE := nat_lt_zero _ _ H4). inversion NE.
     (* single_unfold_list H2. *)
-    pose (EE1 := element_exist Value (length eff) vals H2).
-    pose (EE2 := element_exist Value (length eff) vals0 H1).
-    pose (EE3 := element_exist SideEffectList (length eff) eff6 (eq_sym H3)).
-    pose (EE4 := element_exist Expression x exps (eq_sym H7)).
+    pose (EE1 := element_exist (length eff) vals H2).
+    pose (EE2 := element_exist (length eff) vals0 H1).
+    pose (EE3 := element_exist (length eff) eff6 (eq_sym H3)).
+    pose (EE4 := element_exist x exps (eq_sym H7)).
     inversion EE1 as [v]. inversion EE2 as [v']. inversion EE3 as [fe]. inversion EE4 as [e'].
     inversion H8. inversion H9. inversion H10. inversion H11. subst.
-    pose (EE5 := element_exist _ _ _ (eq_sym H5)).
-    pose (EE6 := element_exist _ _ _ (eq_sym H6)).
+    pose (EE5 := element_exist _ _ (eq_sym H5)).
+    pose (EE6 := element_exist _ _ (eq_sym H6)).
     inversion EE5 as [id']. inversion EE6 as [id''].
     inversion H12. inversion H13. subst.
     assert (0 < Datatypes.length (v' :: x1)). { simpl. omega. }
     pose (P := H0 0 H14).
     assert (0 < Datatypes.length (v :: x0)). { simpl. omega. }
-    pose (P1 := H 0 H15 (inl (nth 0 (v' :: x1) ErrorValue)) (concatn eff1 (fe :: x2) 1) _ P).
-    inversion P1. destruct H17.
-    simpl_concatn_H H17. simpl in H18. apply app_inv_head in H17. inversion H16. subst.
+    pose (P1 := H 0 H15 (inl (nth 0 (v' :: x1) ErrorValue)) (nth_def (fe :: x2) eff1 [] 1) _ P).
+    inversion P1. destruct H17. simpl in H18. inversion H16. simpl in H17. subst.
     
     assert (eff = x2 /\ x0 = x1 /\ x4 = x5).
     {
-      apply IHeff with (exps := x3) (vals := x0) (vals0 := x1) (eff1 := eff1 ++ fe) (id := id''); auto.
+      apply IHeff with (exps := x3) (vals := x0) (vals0 := x1) (eff1 := fe) (id := id''); auto.
       + intros. assert (S j < S (Datatypes.length x0)). { simpl. omega. } pose (P2 := H (S j) H19 v2 eff''). 
-        rewrite concatn_app, concatn_app in P2. simpl in P2. pose (P2 _ H18). assumption.
+        simpl in P2. pose (P2 _ H18). assumption.
       + intros. assert (S j < Datatypes.length (v' :: x1)). { simpl. omega. }
-        pose (P3 := H0 (S j) H18). rewrite concatn_app, concatn_app in P3. simpl in P3. assumption.
+        pose (P3 := H0 (S j) H18). simpl in P3. assumption.
       + inversion H2. inversion H3. inversion H1. auto.
       + inversion H2. inversion H3. inversion H1. auto.
       + intuition.
@@ -592,14 +568,14 @@ forall (exps : list Expression) (vals vals0 : list Value) (eff1 : SideEffectList
 (forall j : nat,
     j < i ->
     forall (v2 : Value + Exception) (eff'' : SideEffectList) (id'' : nat),
-    | env, nth_id ids id j, nth j exps ErrorExp, concatn eff1 eff j | -e> | id'', v2, eff'' | ->
-    inl (nth j vals ErrorValue) = v2 /\ concatn eff1 eff (S j) = eff'' /\ nth_id ids id (S j) = id'')
+    | env, nth_def ids id 0 j, nth j exps ErrorExp, nth_def eff eff1 [] j | -e> | id'', v2, eff'' | ->
+    inl (nth j vals ErrorValue) = v2 /\ nth_def eff eff1 [] (S j) = eff'' /\ nth_def ids id 0 (S j) = id'')
 ->
 (forall j : nat,
      j < i0 ->
-     | env, nth_id ids0 id j, nth j exps ErrorExp, concatn eff1 eff6 j | -e> 
-     | nth_id ids0 id (S j), inl (nth j vals0 ErrorValue),
-     concatn eff1 eff6 (S j) |)
+     | env, nth_def ids0 id 0 j, nth j exps ErrorExp, nth_def eff6 eff1 [] j | -e> 
+     | nth_def ids0 id 0 (S j), inl (nth j vals0 ErrorValue),
+     nth_def eff6 eff1 [] (S j) |)
 ->
 Datatypes.length eff = i ->
 i < Datatypes.length exps ->
@@ -610,51 +586,50 @@ Datatypes.length eff6 = i0 ->
 length ids = i ->
 length ids0 = i0 ->
 i > i0 ->
-(| env, last ids0 id, nth i0 exps ErrorExp, concatn eff1 eff6 i0 | -e> | id', 
-     inr ex0, concatn eff1 eff6 i0 ++ eff4 |)
+(| env, last ids0 id, nth i0 exps ErrorExp, last eff6 eff1 | -e> | id', 
+     inr ex0,eff4 |)
 ->
 False.
 Proof.
 induction eff.
   * intros. simpl in H1. subst. inversion H9.
   * intros. simpl in H1. rewrite <- H1 in H3.
-    pose (EE1 := element_exist Value (length eff) vals (eq_sym H3)).
+    pose (EE1 := element_exist (length eff) vals (eq_sym H3)).
     inversion EE1 as [v]. inversion H11 as [vs]. destruct eff6.
     - subst. apply eq_sym, length_zero_iff_nil in H6. subst. apply length_zero_iff_nil in H8.
       subst.
       simpl in H10. pose (P := H 0 (Nat.lt_0_succ _) _ _ _ H10). inversion P. congruence.
     - subst.
       assert (Datatypes.length ids0 = Datatypes.length vals0) as Helper. { auto. }
-      pose (EE2 := element_exist Value (length eff6) vals0 H6). inversion EE2. inversion H1.
-      pose (NE := nat_exist H2). inversion NE.
-      pose (EE3 := element_exist Expression x1 exps (eq_sym H12)). inversion EE3.
+      pose (EE2 := element_exist (length eff6) vals0 H6). inversion EE2. inversion H1.
+      pose (NE := nat_lt_zero _ _ H2). inversion NE.
+      pose (EE3 := element_exist x1 exps (eq_sym H12)). inversion EE3.
       inversion H13. subst.
-      pose (EE4 := element_exist _ _ _ (eq_sym H7)).
-      pose (EE5 := element_exist _ _ _ (eq_sym H8)).
+      pose (EE4 := element_exist _ _ (eq_sym H7)).
+      pose (EE5 := element_exist _ _ (eq_sym H8)).
       inversion EE4 as [id0']. inversion EE5 as [id0'']. inversion H4. inversion H14. subst.
       assert (s = a /\ id0' = id0''). {
         subst.
         assert (0 < Datatypes.length (x :: x0)). {  simpl. omega. }
         pose (P := H0 0 H15).
         assert (0 < S (Datatypes.length eff)). {  simpl. omega. }
-        pose (P1 := H 0 H16 (inl (nth 0 (x :: x0) ErrorValue)) (concatn eff1 (s :: eff6) 1) _ P).
-        destruct P1. destruct H18.
-        simpl_concatn_H H18. apply app_inv_head in H18. simpl in H19. auto.
+        pose (P1 := H 0 H16 (inl (nth 0 (x :: x0) ErrorValue)) (nth_def (s :: eff6) eff1 [] 1) _ P).
+        destruct P1. destruct H18. simpl in H19, H18. auto.
       }
       destruct H15. subst.
-      eapply IHeff with (exps := x3) (vals := vs) (vals0 := x0) (eff1 := eff1 ++ a) 
+      eapply IHeff with (exps := x3) (vals := vs) (vals0 := x0) (eff1 := a) 
                        (i0 := length eff6) (i := length eff) (ids := x4) (ids0 := x5); auto.
       + intros. assert (S j < S (Datatypes.length eff)). { simpl. omega. }
-        pose (P := H (S j) H17 v2 eff''). rewrite concatn_app, concatn_app in P. simpl in P.
+        pose (P := H (S j) H17 v2 eff''). simpl in P.
         pose (P1 := P _ H16). assumption.
       + intros. inversion H6. assert (S j < Datatypes.length (x :: x0)). { simpl. omega. }
-        pose (P := H0 (S j) H16). rewrite concatn_app, concatn_app in P. simpl in P. assumption.
+        pose (P := H0 (S j) H16). assumption.
       + intuition.
       + inversion H6. auto.
       + rewrite <- H6 in H5. simpl in H5. omega.
       + rewrite <- H6 in Helper. auto.
       + simpl in *. rewrite <- H6 in H9. omega.
-      + rewrite <- last_element_equal in H10. simpl in H10. rewrite concatn_app in H10. 
+      + rewrite <- last_element_equal, <- last_element_equal in H10. simpl in H10. 
         inversion H6. rewrite H16. exact H10.
 Qed.
 
@@ -666,21 +641,21 @@ Lemma exception_equality {env : Environment} {exps : list Expression} (vals vals
 (forall j : nat,
      j < i ->
      forall (v2 : Value + Exception) (eff'' : SideEffectList) (id'' : nat),
-     | env, nth_id ids id j, nth j exps ErrorExp, concatn eff1 eff j | -e> | id'', v2, eff'' | ->
-     inl (nth j vals ErrorValue) = v2 /\ concatn eff1 eff (S j) = eff'' /\ nth_id ids id (S j) = id'')
+     | env, nth_def ids id 0 j, nth j exps ErrorExp, nth_def eff eff1 [] j | -e> | id'', v2, eff'' | ->
+     inl (nth j vals ErrorValue) = v2 /\ nth_def eff eff1 [] (S j) = eff'' /\ nth_def ids id 0 (S j) = id'')
 ->
-| env, last ids0 id, nth i0 exps ErrorExp, concatn eff1 eff6 i0 | -e>
-| id'', inr ex0, concatn eff1 eff6 i0 ++ eff4 |
+| env, last ids0 id, nth i0 exps ErrorExp, last eff6 eff1 | -e>
+| id'', inr ex0, eff4 |
 ->
 (forall (v2 : Value + Exception) (eff'' : SideEffectList) (id'' : nat),
-        | env, last ids id, nth i exps ErrorExp, concatn eff1 eff i | -e>
+        | env, last ids id, nth i exps ErrorExp, last eff eff1 | -e>
         | id'', v2, eff'' | -> inr ex = v2 /\ eff3 = eff'' /\ id' = id'')
 ->
 (forall j : nat,
       j < i0 ->
-      | env, nth_id ids0 id j, nth j exps ErrorExp, concatn eff1 eff6 j | -e>
-      | nth_id ids0 id (S j), inl (nth j vals0 ErrorValue),
-      concatn eff1 eff6 (S j) |)
+      | env, nth_def ids0 id 0 j, nth j exps ErrorExp, nth_def eff6 eff1 [] j | -e>
+      | nth_def ids0 id 0 (S j), inl (nth j vals0 ErrorValue),
+      nth_def eff6 eff1 [] (S j) |)
 ->
 Datatypes.length vals = i ->
  i < Datatypes.length exps ->
@@ -711,18 +686,18 @@ forall {vl : list Expression} (kvals vvals kvals0 vvals0 : list Value) (eff1 : S
 (forall j : nat,
      j < length vl ->
      forall (v2 : Value + Exception) (eff'' : SideEffectList) (id'' : nat),
-     | env, nth_id ids id (2*j), nth j kl ErrorExp, concatn eff1 eff (2 * j) | -e> 
+     | env, nth_def ids id 0 (2*j), nth j kl ErrorExp, nth_def eff eff1 [] (2 * j) | -e> 
      | id'', v2, eff'' | ->
-     inl (nth j kvals ErrorValue) = v2 /\ concatn eff1 eff (S (2 * j)) = eff'' 
-     /\ nth_id ids id (S (2*j)) = id'')
+     inl (nth j kvals ErrorValue) = v2 /\ nth_def eff eff1 [] (S (2 * j)) = eff'' 
+     /\ nth_def ids id 0 (S (2*j)) = id'')
 ->
 (forall j : nat,
      j < length vl ->
      forall (v2 : Value + Exception) (eff'' : SideEffectList) (id'' : nat),
-     | env, nth_id ids id (S (2*j)), nth j vl ErrorExp, concatn eff1 eff (S (2 * j)) | -e> 
+     | env, nth_def ids id 0 (S (2*j)), nth j vl ErrorExp, nth_def eff eff1 [] (S (2 * j)) | -e> 
      | id'', v2, eff'' | ->
-     inl (nth j vvals ErrorValue) = v2 /\ concatn eff1 eff (S (S (2 * j))) = eff'' /\ 
-     nth_id ids id (S (S (2*j))) = id'')
+     inl (nth j vvals ErrorValue) = v2 /\ nth_def eff eff1 [] (S (S (2 * j))) = eff'' /\ 
+     nth_def ids id 0 (S (S (2*j))) = id'')
 ->
 Datatypes.length kl = Datatypes.length vl ->
 length kl = Datatypes.length vvals ->
@@ -731,14 +706,14 @@ length kl = Datatypes.length kvals ->
 ((length kl) * 2)%nat = length ids ->
 (forall j : nat,
       j < length vl ->
-      | env, nth_id ids0 id (2*j), nth j kl ErrorExp, concatn eff1 eff7 (2 * j) | -e> 
-      | nth_id ids0 id (S (2*j)), inl (nth j kvals0 ErrorValue),
-      concatn eff1 eff7 (S (2 * j)) |)
+      | env, nth_def ids0 id 0 (2*j), nth j kl ErrorExp, nth_def eff7 eff1 [] (2 * j) | -e> 
+      | nth_def ids0 id 0 (S (2*j)), inl (nth j kvals0 ErrorValue),
+      nth_def eff7 eff1 [] (S (2 * j)) |)
 ->
 (forall j : nat,
       j < length vl ->
-      | env, nth_id ids0 id (S (2*j)), nth j vl ErrorExp, concatn eff1 eff7 (S (2 * j)) | -e>
-      | nth_id ids0 id (S(S(2*j))), inl (nth j vvals0 ErrorValue), concatn eff1 eff7 (S (S (2 * j))) |)
+      | env, nth_def ids0 id 0 (S (2*j)), nth j vl ErrorExp, nth_def eff7 eff1 [] (S (2 * j)) | -e>
+      | nth_def ids0 id 0 (S(S(2*j))), inl (nth j vvals0 ErrorValue), nth_def eff7 eff1 [] (S (S (2 * j))) |)
 ->
 length kl = Datatypes.length vvals0 ->
 length kl = Datatypes.length kvals0 ->
@@ -749,10 +724,10 @@ kvals = kvals0 /\ vvals = vvals0 /\ eff = eff7 /\ ids = ids0.
 Proof.
   induction kl.
   * intros. inversion H1. inversion H2. inversion H3. inversion H4.
-    repeat unfold_list.
+    repeat empty_list_in_hypo.
     inversion H10. inversion H8. inversion H9. inversion H11. inversion H5.
-    repeat unfold_list.
-    auto.
+    repeat empty_list_in_hypo.
+    subst. auto.
   * intros. inversion H1. inversion H2. inversion H3. inversion H4.
     simpl in H9, H14, H7, H8, H10, H5, H11.
     single_unfold_list. single_unfold_list. single_unfold_list. 
@@ -762,34 +737,31 @@ Proof.
     (** FIRST ELEMENTS ARE EQUAL *)
     pose (F1 := H6 0 (Nat.lt_0_succ (length x7))). simpl in F1.
     pose (F2 := H 0 (Nat.lt_0_succ _) _ _ _ F1). inversion F2. inversion H41.
-    rewrite concatn_app, concatn_app in H43. simpl_concatn_H H43. destruct H43.
-    apply app_inv_head in H43. subst.
+    destruct H43. simpl in H43, H44. subst.
     pose (F3 := H7 0 (Nat.lt_0_succ (length x7))).
     pose (F4 := H0 0 (Nat.lt_0_succ _) _ _ _ F3). inversion F4. inversion H43.
-    rewrite concatn_app, concatn_app in H44. simpl_concatn_H H44. destruct H44.
-    apply app_inv_head in H44. subst. simpl.
+    destruct H44. simpl in H44, H45. subst. simpl.
     (** OTHER ELEMETS *)
     assert (x3 = x15 /\ x5 = x17 /\ x2 = x14 /\ x21 = x11).
     {
       eapply IHkl with (vl := x7); auto.
       * intros. assert (S j < length (x6 :: x7)). { simpl. omega. }
-        pose (P3 := H (S j) H46 v2 eff''). simpl in P3.
-        rewrite concatn_app, concatn_app, concatn_app, Nat.add_0_r, <- plus_n_Sm, concatn_app,
-               <- app_assoc in P3. simpl in H45. rewrite Nat.add_0_r in H45.
+        pose (P3 := H (S j) H46 v2 eff''). simpl mult in H45, P3. rewrite Nat.add_0_r in H45, P3.
+        rewrite Nat.add_succ_r in P3. simpl in P3.
         pose (P4 := P3 _ H45). simpl. rewrite Nat.add_0_r. assumption.
       * intros. assert (S j < length (x6 :: x7)). { simpl. omega. }
-        pose (P3 := H0 (S j) H46 v2 eff''). simpl in P3.
-        rewrite concatn_app, concatn_app, concatn_app, Nat.add_0_r, <- plus_n_Sm, concatn_app,
-               <- app_assoc in P3. simpl in H45. rewrite Nat.add_0_r in H45.
+        pose (P3 := H0 (S j) H46 v2 eff''). simpl mult in H45, P3. rewrite Nat.add_0_r in H45, P3.
+        rewrite Nat.add_succ_r in P3. simpl in P3.
         pose (P4 := P3 _ H45). simpl. rewrite Nat.add_0_r. assumption.
       * intros. assert (S j < length (x6 :: x7)). { simpl. omega. }
-        pose (P3 := H6 (S j) H45). simpl in P3. 
-        rewrite concatn_app, concatn_app, concatn_app, Nat.add_0_r, <- plus_n_Sm, concatn_app,
-               <- app_assoc in P3. simpl. rewrite Nat.add_0_r. assumption.
+        pose (P3 := H6 (S j) H45).
+        simpl. simpl mult in P3. rewrite Nat.add_0_r in P3.
+        rewrite Nat.add_succ_r in P3. simpl in P3. rewrite Nat.add_0_r. assumption.
       * intros. assert (S j < length (x6 :: x7)). { simpl. omega. }
-        pose (P3 := H7 (S j) H45). simpl in P3.
-        rewrite concatn_app, concatn_app, concatn_app, Nat.add_0_r, <- plus_n_Sm, concatn_app,
-               <- app_assoc in P3. simpl. rewrite Nat.add_0_r. assumption.
+        pose (P3 := H7 (S j) H45). 
+        simpl. simpl mult in P3. rewrite Nat.add_0_r in P3.
+        rewrite Nat.add_succ_r in P3. simpl in P3. rewrite Nat.add_0_r. assumption.
+        
     }
     destruct H44. destruct H45. destruct H46. subst. auto.
 Qed.
@@ -802,18 +774,18 @@ Lemma map_lists_equal_until_i {env : Environment} {kl : list Expression} : foral
 (forall j : nat,
      j < length vl ->
      forall (v2 : Value + Exception) (eff'' : SideEffectList) (id'' : nat),
-     | env, nth_id ids id (2*j), nth j kl ErrorExp, concatn eff1 eff (2 * j) | -e>
+     | env, nth_def ids id 0 (2*j), nth j kl ErrorExp, nth_def eff eff1 [] (2 * j) | -e>
      | id'', v2, eff'' | ->
-     inl (nth j kvals ErrorValue) = v2 /\ concatn eff1 eff (S (2 * j)) = eff'' /\
-     nth_id ids id (S (2*j)) = id'')
+     inl (nth j kvals ErrorValue) = v2 /\ nth_def eff eff1 [] (S (2 * j)) = eff'' /\
+     nth_def ids id 0 (S (2*j)) = id'')
 ->
 (forall j : nat,
      j < length vl ->
      forall (v2 : Value + Exception) (eff'' : SideEffectList) (id'' : nat),
-     | env, nth_id ids id (S (2*j)), nth j vl ErrorExp, concatn eff1 eff (S (2 * j)) | -e>
+     | env, nth_def ids id 0 (S (2*j)), nth j vl ErrorExp, nth_def eff eff1 [] (S (2 * j)) | -e>
      | id'', v2, eff'' | ->
-     inl (nth j vvals ErrorValue) = v2 /\ concatn eff1 eff (S (S (2 * j))) = eff'' /\
-     nth_id ids id (S (S (2*j))) = id'')
+     inl (nth j vvals ErrorValue) = v2 /\ nth_def eff eff1 [] (S (S (2 * j))) = eff'' /\
+     nth_def ids id 0 (S (S (2*j))) = id'')
 ->
 Datatypes.length kl = Datatypes.length vl ->
 length kl = Datatypes.length vvals ->
@@ -822,27 +794,27 @@ length kl = Datatypes.length kvals ->
 ((length kl) * 2)%nat = Datatypes.length ids ->
 (forall j : nat,
       j < i0 ->
-      | env, nth_id ids0 id (2*j), nth j kl ErrorExp, concatn eff1 eff7 (2 * j) | -e>
-      | nth_id ids0 id (S (2*j)), inl (nth j kvals0 ErrorValue),
-      concatn eff1 eff7 (S (2 * j)) |)
+      | env, nth_def ids0 id 0 (2*j), nth j kl ErrorExp, nth_def eff7 eff1 [] (2 * j) | -e>
+      | nth_def ids0 id 0 (S (2*j)), inl (nth j kvals0 ErrorValue),
+      nth_def eff7 eff1 [] (S (2 * j)) |)
 ->
 (forall j : nat,
       j < i0 ->
-      | env, nth_id ids0 id (S (2*j)), nth j vl ErrorExp, concatn eff1 eff7 (S (2 * j)) | -e>
-      | nth_id ids0 id (S (S (2*j))), inl (nth j vvals0 ErrorValue), concatn eff1 eff7 (S (S (2 * j))) |)
+      | env, nth_def ids0 id 0 (S (2*j)), nth j vl ErrorExp, nth_def eff7 eff1 [] (S (2 * j)) | -e>
+      | nth_def ids0 id 0 (S (S (2*j))), inl (nth j vvals0 ErrorValue), nth_def eff7 eff1 [] (S (S (2 * j))) |)
 ->
 Datatypes.length vvals0 = i0 ->
 Datatypes.length kvals0 = i0 ->
 i0 <= Datatypes.length kl ->
 Datatypes.length eff7 = (i0 * 2)%nat ->
 length ids0 = (i0 * 2)%nat ->
-(| env, last ids0 id, nth i0 kl ErrorExp, concatn eff1 eff7 (2 * i0) | -e>
-| id', inr ex0, concatn eff1 eff7 (2 * i0) ++ eff5 |
+(| env, last ids0 id, nth i0 kl ErrorExp, last eff7 eff1 | -e>
+| id', inr ex0, eff5 |
 \/
-(| env, last ids0 id, nth i0 kl ErrorExp, concatn eff1 eff7 (2 * i0) | -e> | id', inl val0,
-      concatn eff1 eff7 (2 * i0) ++ eff5 | /\
-| env, id', nth i0 vl ErrorExp, concatn eff1 eff7 (2 * i0) ++ eff5 | -e> | 
-      id'', inr ex0, concatn eff1 eff7 (2 * i0) ++ eff5 ++ eff6 |)
+(| env, last ids0 id, nth i0 kl ErrorExp, last eff7 eff1 | -e> | id', inl val0,
+      eff5 | /\
+| env, id', nth i0 vl ErrorExp, eff5 | -e> | 
+      id'', inr ex0, eff6 |)
 )
 ->
 length vl = i0 /\ kvals = kvals0 /\ vvals = vvals0 /\ eff = eff7 /\ ids = ids0.
@@ -855,7 +827,7 @@ Proof.
     inversion H4. apply eq_sym, length_zero_iff_nil in H14. subst. apply length_zero_iff_nil in H9.
     subst. apply eq_sym, length_zero_iff_nil in H5. auto.
   * intros. inversion H1.
-    pose (EE1 := element_exist Expression (length kl) vl H15). 
+    pose (EE1 := element_exist (length kl) vl H15). 
     inversion EE1 as [ve]. inversion H14 as [ves].
     subst.
     case_eq (length vvals0).
@@ -863,75 +835,73 @@ Proof.
       apply length_zero_iff_nil in H9. apply length_zero_iff_nil in H12.
       apply length_zero_iff_nil in H11. subst.
       rewrite <- H1 in H, H0.
-      simpl_concatn_H H13.
       inversion H13.
-      + pose (P1 := H 0 (Nat.lt_0_succ _) (inr ex0) (eff1 ++ eff5) id').
-        simpl_concatn_H P1. pose (P2 := P1 H8). inversion P2. inversion H9.
-      + destruct H8. pose (P1 := H 0 (Nat.lt_0_succ _) (inl val0) (eff1 ++ eff5) id').
-        simpl_concatn_H P1. pose (P2 := P1 H8). destruct P2. inversion H11. subst.
-        pose (P3 := H0 0 (Nat.lt_0_succ _) (inr ex0) (eff1 ++ eff5 ++ eff6) id'').
-        simpl_concatn_H P3.
+      + pose (P1 := H 0 (Nat.lt_0_succ _) (inr ex0) ( eff5) id').
+        simpl in P1, H8.
+        pose (P2 := P1 H8). inversion P2. inversion H9.
+      + destruct H8. pose (P1 := H 0 (Nat.lt_0_succ _) (inl val0) (eff5) id').
+        pose (P2 := P1 H8). destruct P2. inversion H11. subst.
+        pose (P3 := H0 0 (Nat.lt_0_succ _) (inr ex0) (eff6) id'').
         destruct H12.
         rewrite <- H12 in H9 at 1. rewrite H16 in P3.
         pose (P4 := P3 H9). inversion P4. inversion H17.
 
     - intros. rewrite H8 in *. simpl in H2, H3. simpl in H4, H10.
-      pose (EE2 := element_exist Value _ kvals0 (eq_sym H9)).
-      pose (EE3 := element_exist Value _ vvals0 (eq_sym H8)).
-      pose (EE4 := element_exist Value _ kvals H3).
-      pose (EE5 := element_exist Value _ vvals H2).
-      pose (EE6 := element_exist SideEffectList _ eff H4).
-      pose (EE7 := element_exist SideEffectList _ eff7 (eq_sym H11)).
-      pose (EE8 := element_exist _ _ _ H5).
-      pose (EE9 := element_exist _ _ _ (eq_sym H12)).
+      pose (EE2 := element_exist _ kvals0 (eq_sym H9)).
+      pose (EE3 := element_exist _ vvals0 (eq_sym H8)).
+      pose (EE4 := element_exist _ kvals H3).
+      pose (EE5 := element_exist _ vvals H2).
+      pose (EE6 := element_exist _ eff H4).
+      pose (EE7 := element_exist _ eff7 (eq_sym H11)).
+      pose (EE8 := element_exist _ _ H5).
+      pose (EE9 := element_exist _ _ (eq_sym H12)).
       inversion EE2 as [kv']. inversion EE3 as [vv']. inversion EE4 as [kv]. inversion EE5 as [vv].
       inversion EE6 as [e1]. inversion EE7 as [e1']. inversion EE8 as [id1]. inversion EE9 as [id1'].
       inversion H16. inversion H17. inversion H18. inversion H19.
       inversion H20. inversion H21. inversion H22. inversion H23. subst.
       
       inversion H4. inversion H11. inversion H5. inversion H12.
-      pose (EE10 := element_exist SideEffectList _ x3 (H25)).
-      pose (EE11 := element_exist SideEffectList _ x4 (eq_sym H26)).
-      pose (EE12 := element_exist _ _ x5 (H27)).
-      pose (EE13 := element_exist _ _ x6 (eq_sym H28)).
+      pose (EE10 := element_exist _ x3 (H25)).
+      pose (EE11 := element_exist _ x4 (eq_sym H26)).
+      pose (EE12 := element_exist _ x5 (H27)).
+      pose (EE13 := element_exist _ x6 (eq_sym H28)).
       inversion EE10 as [e2]. inversion EE11 as [e2']. inversion EE12 as [id2]. inversion EE13 as [id2']. 
       inversion H24. inversion H29. inversion H30. inversion H31. subst.
       (** FIRST ELEMENTS ARE EQUAL *)
       pose (F1 := H6 0 (Nat.lt_0_succ n)).
       pose (F2 := H 0 (Nat.lt_0_succ _) _ _ _ F1). inversion F2. inversion H32. destruct H33.
-      rewrite concatn_app, concatn_app in H33. simpl_concatn_H H33. apply app_inv_head in H33. 
-      simpl in H34. subst.
+      simpl in H34, H33. subst.
       pose (F3 := H7 0 (Nat.lt_0_succ n)).
       pose (F4 := H0 0 (Nat.lt_0_succ _) _ _ _ F3). inversion F4. inversion H33. destruct H34.
-      rewrite concatn_app, concatn_app in H34. simpl_concatn_H H34. apply app_inv_head in H34. 
-      simpl in H35. subst. simpl.
+      simpl in H35, H34. subst. simpl.
       (** OTHER ELEMETS *)
       assert (length ves = n /\ x1 = x /\ x2 = x0 /\ x7 = x8 /\ x9 = x10).
       {
-        eapply IHkl with (eff1 := eff1 ++ e1' ++ e2') (ex0 := ex0) (eff5 := eff5) (vl := ves)
+        eapply IHkl with (* (eff1 := eff1 ++ e1' ++ e2') *) (ex0 := ex0) (eff5 := eff5) (vl := ves)
                          (eff6 := eff6) (val0 := val0); auto.
         * intros. assert (S j < length (ve :: ves)). { simpl. omega. }
-          pose (P3 := H (S j) H36 v2 eff''). simpl in P3.
-          rewrite concatn_app, concatn_app, concatn_app, Nat.add_0_r,
-                <- plus_n_Sm, concatn_app, <- app_assoc in P3. simpl in H35. rewrite Nat.add_0_r in H35.
+          pose (P3 := H (S j) H36 v2 eff''). simpl mult in H35, P3. rewrite Nat.add_0_r in H35, P3.
+          rewrite Nat.add_succ_r in P3. simpl in P3.
           pose (P4 := P3 _ H35). simpl. rewrite Nat.add_0_r. assumption.
         * intros. assert (S j < length (ve :: ves)). { simpl. omega. }
-          pose (P3 := H0 (S j) H36 v2 eff''). simpl in P3.
-          rewrite concatn_app, concatn_app, concatn_app, Nat.add_0_r,
-                <- plus_n_Sm, concatn_app, <- app_assoc in P3. simpl in H35. rewrite Nat.add_0_r in H35.
+          pose (P3 := H0 (S j) H36 v2 eff''). 
+          simpl mult in H35, P3. rewrite Nat.add_0_r in H35, P3.
+          rewrite Nat.add_succ_r in P3. simpl in P3.
           pose (P4 := P3 _ H35). simpl. rewrite Nat.add_0_r. assumption.
         * intros. assert (S j < S n). { omega. }
           pose (P3 := H6 (S j) H35). simpl in P3.
-          rewrite concatn_app, concatn_app, concatn_app, Nat.add_0_r,
-                <- plus_n_Sm, concatn_app, <- app_assoc in P3. simpl. rewrite Nat.add_0_r. assumption.
+          simpl mult in P3. rewrite Nat.add_0_r in P3.
+          rewrite Nat.add_succ_r in P3. simpl in P3.
+          simpl. rewrite Nat.add_0_r. assumption.
         * intros. assert (S j < S n). { omega. }
           pose (P3 := H7 (S j) H35). simpl in P3.
-          rewrite concatn_app, concatn_app, concatn_app, Nat.add_0_r,
-               <- plus_n_Sm, concatn_app, <- app_assoc in P3. simpl. rewrite Nat.add_0_r. assumption.
+          simpl mult in *. rewrite Nat.add_0_r in *.
+          rewrite Nat.add_succ_r in *. simpl in *.
+          assumption.
         * simpl in H9. omega.
-        * rewrite <- last_element_equal, <- last_element_equal in H13. simpl in H13.
-          rewrite concatn_app, Nat.add_0_r, <- plus_n_Sm, concatn_app,
-              <- app_assoc in H13. simpl. rewrite Nat.add_0_r. exact H13.
+        * rewrite <- last_element_equal, <- last_element_equal,
+                  <- last_element_equal, <- last_element_equal in H13. simpl in H13.
+          simpl. exact H13.
       }
       destruct H34. destruct H35. destruct H36. destruct H37. subst. auto.
 Qed.
@@ -945,21 +915,21 @@ Lemma map_lists_equal_until_i_key {env : Environment} {kl : list Expression} :
 (forall j : nat,
      j < i ->
      forall (v2 : Value + Exception) (eff'' : SideEffectList) (id'' : nat),
-     | env, nth_id ids id (2 * j), nth j kl ErrorExp, concatn eff1 eff (2 * j) | -e> | id'', v2, eff'' | ->
-     inl (nth j kvals ErrorValue) = v2 /\ concatn eff1 eff (S (2 * j)) = eff'' /\
-     nth_id ids id (S (2 * j)) = id'')
+     | env, nth_def ids id 0 (2 * j), nth j kl ErrorExp, nth_def eff eff1 [] (2 * j) | -e> | id'', v2, eff'' | ->
+     inl (nth j kvals ErrorValue) = v2 /\ nth_def eff eff1 [] (S (2 * j)) = eff'' /\
+     nth_def ids id 0 (S (2 * j)) = id'')
 ->
 (forall j : nat,
      j < i ->
      forall (v2 : Value + Exception) (eff'' : SideEffectList) (id'' : nat),
-     | env, nth_id ids id (S (2 * j)), nth j vl ErrorExp, concatn eff1 eff (S (2 * j)) | -e>
+     | env, nth_def ids id 0 (S (2 * j)), nth j vl ErrorExp, nth_def eff eff1 [] (S (2 * j)) | -e>
      | id'', v2, eff'' | ->
-     inl (nth j vvals ErrorValue) = v2 /\ concatn eff1 eff (S (S (2 * j))) = eff'' /\
-     nth_id ids id (S (S (2 * j))) = id'')
+     inl (nth j vvals ErrorValue) = v2 /\ nth_def eff eff1 [] (S (S (2 * j))) = eff'' /\
+     nth_def ids id 0 (S (S (2 * j))) = id'')
 ->
 (forall (v2 : Value + Exception) (eff'' : SideEffectList) (id'' : nat),
-         | env, last ids id, nth i kl ErrorExp, concatn eff1 eff (2 * i) | -e> | id'', v2, eff'' | ->
-         inr ex = v2 /\ concatn eff1 eff (2 * i) ++ eff2 = eff'' /\ id1 = id'')
+         | env, last ids id, nth i kl ErrorExp, last eff eff1 | -e> | id'', v2, eff'' | ->
+         inr ex = v2 /\ eff2 = eff'' /\ id1 = id'')
 ->
 Datatypes.length kl = Datatypes.length vl ->
 Datatypes.length vvals = i ->
@@ -969,28 +939,28 @@ Datatypes.length eff = (i * 2)%nat ->
 length ids = (i*2)%nat ->
 (forall j : nat,
       j < i0 ->
-      | env, nth_id ids0 id (2 * j), nth j kl ErrorExp, concatn eff1 eff7 (2 * j) | -e>
-      | nth_id ids0 id (S (2 * j)), inl (nth j kvals0 ErrorValue),
-      concatn eff1 eff7 (S (2 * j)) |)
+      | env, nth_def ids0 id 0 (2 * j), nth j kl ErrorExp, nth_def eff7 eff1 [] (2 * j) | -e>
+      | nth_def ids0 id 0 (S (2 * j)), inl (nth j kvals0 ErrorValue),
+      nth_def eff7 eff1 [] (S (2 * j)) |)
 ->
 (forall j : nat,
   j < i0 ->
-  | env, nth_id ids0 id (S (2 * j)), nth j vl ErrorExp, concatn eff1 eff7 (S (2 * j)) | -e>
-  | nth_id ids0 id (S (S (2 * j))), inl (nth j vvals0 ErrorValue), concatn eff1 eff7 (S (S (2 * j))) |)
+  | env, nth_def ids0 id 0 (S (2 * j)), nth j vl ErrorExp, nth_def eff7 eff1 [] (S (2 * j)) | -e>
+  | nth_def ids0 id 0 (S (S (2 * j))), inl (nth j vvals0 ErrorValue), nth_def eff7 eff1 [] (S (S (2 * j))) |)
 ->
 Datatypes.length vvals0 = i0 ->
 Datatypes.length kvals0 = i0 ->
 i0 <= Datatypes.length kl ->
 Datatypes.length eff7 = (i0 * 2)%nat ->
 length ids0 = (i0*2)%nat ->
-(| env, last ids0 id, nth i0 kl ErrorExp, concatn eff1 eff7 (2 * i0) | -e>
-| id1', inr ex0, concatn eff1 eff7 (2 * i0) ++ eff5 |
+(| env, last ids0 id, nth i0 kl ErrorExp, last eff7 eff1 | -e>
+| id1', inr ex0, eff5 |
 \/
-(| env, last ids0 id, nth i0 kl ErrorExp, concatn eff1 eff7 (2 * i0) | -e>
+(| env, last ids0 id, nth i0 kl ErrorExp, last eff7 eff1 | -e>
 | id1', inl val0,
-      concatn eff1 eff7 (2 * i0) ++ eff5 | /\
-| env, id1', nth i0 vl ErrorExp, concatn eff1 eff7 (2 * i0) ++ eff5 | -e> | 
-      id2', inr ex0, concatn eff1 eff7 (2 * i0) ++ eff5 ++ eff6 |)
+       eff5 | /\
+| env, id1', nth i0 vl ErrorExp, eff5 | -e> | 
+      id2', inr ex0, eff6 |)
 )
 ->
 i = i0 /\ kvals = kvals0 /\ vvals = vvals0 /\ eff = eff7 /\ ids = ids0.
@@ -1007,7 +977,7 @@ Proof.
     inversion H14. apply length_zero_iff_nil in H10. subst. 
     auto.
   * intros. inversion H2.
-    pose (EE1 := element_exist Expression (length kl) vl H17).
+    pose (EE1 := element_exist (length kl) vl H17).
     inversion EE1 as [ve]. inversion H16 as [ves]. subst.
     case_eq (length vvals); case_eq (length vvals0).
     - intros.
@@ -1022,54 +992,55 @@ Proof.
       subst. auto.
     - intros. rewrite H3, H10 in *.
       apply length_zero_iff_nil in H6.
-      pose (EE2 := element_exist SideEffectList _ eff7 (eq_sym H13)).
+      pose (EE2 := element_exist _ eff7 (eq_sym H13)).
       inversion EE2. inversion H18.
       subst. inversion H13. 
-      pose (EE3 := element_exist SideEffectList _ x0 (eq_sym H19)).
+      pose (EE3 := element_exist _ x0 (eq_sym H19)).
       inversion EE3. inversion H6.
       apply length_zero_iff_nil in H7. subst.
       pose (P1 := H8 0 (Nat.lt_0_succ n)). pose (P2 := H9 0 (Nat.lt_0_succ n)). simpl in P1, P2.
       pose (P3 := H1 _ _ _ P1). inversion P3.
       inversion H7.
-    - intros. rewrite H3, H10 in *. simpl_concatn_H H15.
+    - intros. rewrite H3, H10 in *.
       inversion H15.
       (** KEY EXCEPTION *)
-        + pose (P2 := H 0 (Nat.lt_0_succ n) (inr ex0) (eff1 ++ eff5)).
+        + pose (P2 := H 0 (Nat.lt_0_succ n) (inr ex0) (eff5)).
           apply length_zero_iff_nil in H14. subst.
-          simpl_concatn_H P2. pose (P3 := P2 _ H18). inversion P3. inversion H14.
+          apply length_zero_iff_nil in H13. subst.
+          simpl in P2, H18.
+          pose (P3 := P2 _ H18). inversion P3. inversion H13.
       (** VALUE EXCEPTION *)
         + destruct H18.
-          pose (P2 := H 0 (Nat.lt_0_succ n) (inl val0) (eff1 ++ eff5)).
-          simpl_concatn_H P2.
+          pose (P2 := H 0 (Nat.lt_0_succ n) (inl val0) (eff5)).
           apply length_zero_iff_nil in H14. subst.
+          apply length_zero_iff_nil in H13. subst.
+          simpl in P2, H18.
           pose (P3 := P2 _ H18).
           inversion P3.
-          pose (P4 := H0 0 (Nat.lt_0_succ n) (inr ex0) (eff1 ++ eff5 ++ eff6)). simpl in P4.
-          destruct H20. subst.
-          assert (concatn eff1 eff 1 = eff1 ++ eff5). { simpl_concatn. exact H20. }
-          rewrite H21 in P4. rewrite <- app_assoc in H19.
+          pose (P4 := H0 0 (Nat.lt_0_succ n) (inr ex0) (eff6)). simpl in P4.
+          destruct H14. subst.
           pose (P5 := P4 _ H19).
-          inversion P5. inversion H22.
+          inversion P5. inversion H14.
 
     - intros. rewrite H3, H10 in *.
-      pose (EE2 := element_exist Value n kvals0 (eq_sym H11)).
-      pose (EE3 := element_exist Value n vvals0 (eq_sym H3)).
-      pose (EE4 := element_exist Value n0 kvals (eq_sym H4)).
-      pose (EE5 := element_exist Value n0 vvals (eq_sym H10)).
-      pose (EE6 := element_exist SideEffectList _ eff (eq_sym H6)).
-      pose (EE7 := element_exist SideEffectList _ eff7 (eq_sym H13)).
-      pose (EE8 := element_exist _ _ _ (eq_sym H7)).
-      pose (EE9 := element_exist _ _ _ (eq_sym H14)).
+      pose (EE2 := element_exist n kvals0 (eq_sym H11)).
+      pose (EE3 := element_exist n vvals0 (eq_sym H3)).
+      pose (EE4 := element_exist n0 kvals (eq_sym H4)).
+      pose (EE5 := element_exist n0 vvals (eq_sym H10)).
+      pose (EE6 := element_exist _ eff (eq_sym H6)).
+      pose (EE7 := element_exist _ eff7 (eq_sym H13)).
+      pose (EE8 := element_exist _ _ (eq_sym H7)).
+      pose (EE9 := element_exist _ _ (eq_sym H14)).
       inversion EE2 as [kv']. inversion EE3 as [vv']. inversion EE4 as [kv]. 
       inversion EE5 as [vv]. inversion EE6 as [e1]. inversion EE7 as [e1'].
       inversion EE8 as [id01]. inversion EE9 as [id01'].
       inversion H18. inversion H19. inversion H20. inversion H21.
       inversion H22. inversion H23. inversion H24. inversion H25. subst.
       inversion H6. inversion H13. inversion H7. inversion H14.
-      pose (EE10 := element_exist SideEffectList _ x3 (eq_sym H27)).
-      pose (EE11 := element_exist SideEffectList _ x4 (eq_sym H28)).
-      pose (EE12 := element_exist _ _ x5 (eq_sym H29)).
-      pose (EE13 := element_exist _ _ x6 (eq_sym H30)).
+      pose (EE10 := element_exist _ x3 (eq_sym H27)).
+      pose (EE11 := element_exist _ x4 (eq_sym H28)).
+      pose (EE12 := element_exist _ x5 (eq_sym H29)).
+      pose (EE13 := element_exist _ x6 (eq_sym H30)).
       inversion EE10 as [e2]. inversion EE11 as [e2'].
       inversion EE12 as [id02]. inversion EE13 as [id02'].
       inversion H26. inversion H31. inversion H32. inversion H33. subst.
@@ -1079,56 +1050,48 @@ Proof.
       pose (F1 := H8 0 (Nat.lt_0_succ n)).
       pose (F2 := H 0 (Nat.lt_0_succ n0) _ _ _ F1). inversion F2. inversion H34.
       destruct H35. simpl in H36.
-      rewrite concatn_app, concatn_app in H35. simpl_concatn_H H35. apply app_inv_head in H35. subst.
+      simpl in H35. subst.
       pose (F3 := H9 0 (Nat.lt_0_succ n)).
       pose (F4 := H0 0 (Nat.lt_0_succ n0) _ _ _ F3). inversion F4. inversion H35.
       destruct H36. simpl in H37.
-      rewrite concatn_app, concatn_app in H36. simpl_concatn_H H36. apply app_inv_head in H36. subst.
+      simpl in H36. subst.
       (** OTHER ELEMETS *)
       assert (n0 = n /\ x1 = x /\ x2 = x0 /\ x7 = x8 /\ x9 = x10).
       {
-        eapply IHkl with (eff1 := eff1 ++ e1' ++ e2') (ex0 := ex0) (eff5 := eff5) (eff2 := eff2) 
+        eapply IHkl with (* (eff1 := eff1 ++ e1' ++ e2') *) (ex0 := ex0) (eff5 := eff5) (eff2 := eff2) 
                         (ex := ex) (vl := ves) (eff6 := eff6) (val0 := val0); auto.
         * intros. assert (S j < S n0). { omega. } pose (P3 := H (S j) H38 v2 eff'').
-          simpl in P3.
-          rewrite concatn_app, concatn_app, concatn_app, Nat.add_0_r,
-               <- plus_n_Sm, concatn_app, <- app_assoc in P3. simpl in H37. rewrite Nat.add_0_r in H37.
+          simpl mult in H37, P3. rewrite Nat.add_0_r in H37, P3.
+          rewrite Nat.add_succ_r in P3. simpl in P3.
           pose (P4 := P3 _ H37). simpl. rewrite Nat.add_0_r. assumption.
         * intros. assert (S j < S n0). { omega. }
           pose (P3 := H0 (S j) H38 v2 eff''). simpl in P3.
-          rewrite concatn_app, concatn_app, concatn_app, Nat.add_0_r,
-               <- plus_n_Sm, concatn_app, <- app_assoc in P3. simpl in H37. rewrite Nat.add_0_r in H37.
+          simpl mult in H37, P3. rewrite Nat.add_0_r in H37, P3.
+          rewrite Nat.add_succ_r in P3. simpl in P3.
           pose (P4 := P3 _ H37). simpl. rewrite Nat.add_0_r. assumption.
         * intros. pose (P3 := H1 v2 eff'').
-          rewrite <- last_element_equal, <- last_element_equal in P3. simpl in P3.
-          rewrite concatn_app, Nat.add_0_r, <- plus_n_Sm, concatn_app, <- app_assoc in P3.
-          simpl. rewrite Nat.add_0_r. simpl in H36. rewrite Nat.add_0_r in H36. apply (P3 _ H36).
+          rewrite <- last_element_equal, <- last_element_equal,
+                  <- last_element_equal, <- last_element_equal in P3. simpl in P3.
+          simpl.
+          simpl mult in P3.
+          apply (P3 _ H36).
         * simpl in H5. omega.
         * intros. assert (S j < S n). { omega. }
-          pose (P3 := H8 (S j) H37). simpl in P3.
-          rewrite Nat.add_0_r, concatn_app, concatn_app, concatn_app,
-               <- plus_n_Sm, concatn_app, <- app_assoc in P3. simpl. rewrite Nat.add_0_r. assumption.
+          pose (P3 := H8 (S j) H37). simpl mult in P3. rewrite Nat.add_0_r in P3.
+          rewrite Nat.add_succ_r in P3. simpl in P3.
+          simpl. rewrite Nat.add_0_r. assumption.
         * intros. assert (S j < S n). { omega. }
-        pose (P3 := H9 (S j) H37).
-          simpl in P3. 
-          rewrite concatn_app, concatn_app, concatn_app, Nat.add_0_r,
-               <- plus_n_Sm, concatn_app, <- app_assoc in P3. simpl. rewrite Nat.add_0_r. assumption.
+          pose (P3 := H9 (S j) H37).
+          simpl mult in P3. rewrite Nat.add_0_r in P3.
+          rewrite Nat.add_succ_r in P3. simpl in P3.
+          simpl. rewrite Nat.add_0_r. assumption.
         * simpl in H11. omega.
-        * rewrite <- last_element_equal, <- last_element_equal in H15.
-          simpl in H15. 
-          rewrite concatn_app, Nat.add_0_r, <- plus_n_Sm, concatn_app,
-               <- app_assoc in H15. simpl. rewrite Nat.add_0_r.
+        * rewrite <- last_element_equal, <- last_element_equal,
+                  <- last_element_equal, <- last_element_equal in H15.
           exact H15.
       }
       destruct H36. destruct H37. destruct H38. destruct H39. subst. auto.
 Qed.
-
-Ltac simpl_concatn_app Hyp :=
-repeat (rewrite Nat.add_0_r in Hyp);
-repeat (rewrite plus_n_Sm in Hyp);
-repeat (rewrite concatn_app in Hyp);
-repeat (rewrite app_assoc in Hyp)
-.
 
 (** Map lists are equal until ith value *)
 Lemma map_lists_equal_until_i_val {env : Environment} {kl : list Expression} : 
@@ -1139,23 +1102,23 @@ Lemma map_lists_equal_until_i_val {env : Environment} {kl : list Expression} :
 (forall j : nat,
      j < i ->
      forall (v2 : Value + Exception) (eff'' : SideEffectList) (id'' : nat),
-     | env, nth_id ids id (2*j), nth j kl ErrorExp, concatn eff1 eff (2 * j) | -e> | id'', v2, eff'' | ->
-     inl (nth j kvals ErrorValue) = v2 /\ concatn eff1 eff (S (2 * j)) = eff'' /\
-     nth_id ids id (S (2*j)) = id'')
+     | env, nth_def ids id 0 (2*j), nth j kl ErrorExp, nth_def eff eff1 [] (2 * j) | -e> | id'', v2, eff'' | ->
+     inl (nth j kvals ErrorValue) = v2 /\ nth_def eff eff1 [] (S (2 * j)) = eff'' /\
+     nth_def ids id 0 (S (2*j)) = id'')
 ->
 (forall j : nat,
      j < i ->
      forall (v2 : Value + Exception) (eff'' : SideEffectList) (id'' : nat),
-     | env, nth_id ids id (S (2*j)), nth j vl ErrorExp, concatn eff1 eff (S (2 * j)) | -e> | id'', v2, eff'' | ->
-     inl (nth j vvals ErrorValue) = v2 /\ concatn eff1 eff (S (S (2 * j))) = eff'' /\
-     nth_id ids id (S (S (2*j))) = id'')
+     | env, nth_def ids id 0 (S (2*j)), nth j vl ErrorExp, nth_def eff eff1 [] (S (2 * j)) | -e> | id'', v2, eff'' | ->
+     inl (nth j vvals ErrorValue) = v2 /\ nth_def eff eff1 [] (S (S (2 * j))) = eff'' /\
+     nth_def ids id 0 (S (S (2*j))) = id'')
 ->
 (forall (v2 : Value + Exception) (eff'' : SideEffectList) (id'' : nat),
-         | env, last ids id, nth i kl ErrorExp, concatn eff1 eff (2 * i) | -e> | id'', v2, eff'' | ->
-         inl val = v2 /\ concatn eff1 eff (2 * i) ++ eff2 = eff'' /\ id1 = id'')
+         | env, last ids id, nth i kl ErrorExp, last eff eff1 | -e> | id'', v2, eff'' | ->
+         inl val = v2 /\ eff2 = eff'' /\ id1 = id'')
 ->
 (forall (v2 : Value + Exception) (eff'' : SideEffectList) (id'' : nat),
-         | env, id1, nth i vl ErrorExp, concatn eff1 eff (2 * i) ++ eff2 | -e> | id'', v2, eff'' | ->
+         | env, id1, nth i vl ErrorExp, eff2 | -e> | id'', v2, eff'' | ->
          inr ex = v2 /\ eff4 = eff'' /\ id2 = id'')
 ->
 Datatypes.length kl = Datatypes.length vl ->
@@ -1166,27 +1129,27 @@ Datatypes.length eff = (i * 2)%nat ->
 Datatypes.length ids = (i * 2)%nat ->
 (forall j : nat,
       j < i0 ->
-      | env, nth_id ids0 id (2*j), nth j kl ErrorExp, concatn eff1 eff7 (2 * j) | -e>
-      | nth_id ids0 id (S (2*j)), inl (nth j kvals0 ErrorValue),
-      concatn eff1 eff7 (S (2 * j)) |)
+      | env, nth_def ids0 id 0 (2*j), nth j kl ErrorExp, nth_def eff7 eff1 [] (2 * j) | -e>
+      | nth_def ids0 id 0 (S (2*j)), inl (nth j kvals0 ErrorValue),
+      nth_def eff7 eff1 [] (S (2 * j)) |)
 ->
 (forall j : nat,
   j < i0 ->
-  | env, nth_id ids0 id (S (2*j)), nth j vl ErrorExp, concatn eff1 eff7 (S (2 * j)) | -e>
-  | nth_id ids0 id (S (S (2*j))), inl (nth j vvals0 ErrorValue), concatn eff1 eff7 (S (S (2 * j))) |)
+  | env, nth_def ids0 id 0 (S (2*j)), nth j vl ErrorExp, nth_def eff7 eff1 [] (S (2 * j)) | -e>
+  | nth_def ids0 id 0 (S (S (2*j))), inl (nth j vvals0 ErrorValue), nth_def eff7 eff1 [] (S (S (2 * j))) |)
 ->
 Datatypes.length vvals0 = i0 ->
 Datatypes.length kvals0 = i0->
 i0 <= Datatypes.length kl ->
 Datatypes.length eff7 = (i0 * 2)%nat ->
 Datatypes.length ids0 = (i0 * 2)%nat ->
-(| env, last ids0 id, nth i0 kl ErrorExp, concatn eff1 eff7 (2 * i0) | -e>
-| id1', inr ex0, concatn eff1 eff7 (2 * i0) ++ eff5 |
+(| env, last ids0 id, nth i0 kl ErrorExp, last eff7 eff1 | -e>
+| id1', inr ex0, eff5 |
 \/
-(| env, last ids0 id, nth i0 kl ErrorExp, concatn eff1 eff7 (2 * i0) | -e> | id1', inl val0,
-      concatn eff1 eff7 (2 * i0) ++ eff5 | /\
-| env, id1', nth i0 vl ErrorExp, concatn eff1 eff7 (2 * i0) ++ eff5 | -e> | 
-      id2', inr ex0, concatn eff1 eff7 (2 * i0) ++ eff5 ++ eff6 |)
+(| env, last ids0 id, nth i0 kl ErrorExp, last eff7 eff1 | -e> | id1', inl val0,
+      eff5 | /\
+| env, id1', nth i0 vl ErrorExp, eff5 | -e> | 
+      id2', inr ex0, eff6 |)
 )
 ->
 i = i0 /\ kvals = kvals0 /\ vvals = vvals0 /\ eff = eff7 /\ ids = ids0.
@@ -1204,7 +1167,7 @@ Proof.
     inversion H12. apply length_zero_iff_nil in H11. subst.
     auto.
   * intros. inversion H3.
-    pose (EE1 := element_exist Expression (length kl) vl H18).
+    pose (EE1 := element_exist (length kl) vl H18).
     inversion EE1 as [ve]. inversion H17 as [ves]. subst.
     case_eq (length vvals); case_eq (length vvals0).
     - intros.
@@ -1219,58 +1182,57 @@ Proof.
       subst. auto.
     - intros. rewrite H4, H11 in *.
       apply length_zero_iff_nil in H7.
-      pose (EE2 := element_exist SideEffectList _ eff7 (eq_sym H14)).
+      pose (EE2 := element_exist _ eff7 (eq_sym H14)).
       inversion EE2. inversion H19. subst.
       inversion H14. 
-      pose (EE3 := element_exist SideEffectList _ x0 (eq_sym H20)). 
+      pose (EE3 := element_exist _ x0 (eq_sym H20)). 
       inversion EE3. inversion H7.
       subst.
       pose (P1 := H9 0 (Nat.lt_0_succ n)).
       pose (P2 := H10 0 (Nat.lt_0_succ n)). simpl in P1, P2.
       apply length_zero_iff_nil in H8. subst.
       pose (P3 := H1 _ _ _ P1). inversion P3.
-      inversion H8. destruct H21. rewrite concatn_app in H21. simpl_concatn_H H21.
-      apply app_inv_head in H21. simpl in H22. subst.
-      simpl_concatn_H H2. simpl_concatn_H P2.
+      inversion H8. destruct H21. subst.
       pose (P4 := H2 _ _ _ P2). inversion P4. inversion H21.
-    - intros. rewrite H4, H11 in *. simpl_concatn_H H16.
+    - intros. rewrite H4, H11 in *.
       inversion H16.
       (** KEY EXCEPTION *)
-        + pose (P2 := H 0 (Nat.lt_0_succ n) (inr ex0) (eff1 ++ eff5)).
+        + pose (P2 := H 0 (Nat.lt_0_succ n) (inr ex0) (eff5)).
           apply length_zero_iff_nil in H15. subst.
-          simpl_concatn_H P2. pose (P3 := P2 _ H19). inversion P3. inversion H15.
+          apply length_zero_iff_nil in H14. subst.
+          simpl in P2, H19.
+          pose (P3 := P2 _ H19). inversion P3. inversion H14.
       (** VALUE EXCEPTION *)
-        + pose (P2 := H 0 (Nat.lt_0_succ n) (inl val0) (eff1 ++ eff5)).
+        + pose (P2 := H 0 (Nat.lt_0_succ n) (inl val0) (eff5)).
           apply length_zero_iff_nil in H15. subst.
-          simpl_concatn_H P2.
-          destruct H19. pose (P3 := P2 _ H15).
-          inversion P3. destruct H21. subst.
-          pose (P4 := H0 0 (Nat.lt_0_succ n) (inr ex0) (eff1 ++ eff5 ++ eff6)).
+          apply length_zero_iff_nil in H14. subst.
+          destruct H19.
+          pose (P3 := P2 _ H14).
+          inversion P3. destruct H20. subst.
+          pose (P4 := H0 0 (Nat.lt_0_succ n) (inr ex0) (eff6)).
           simpl in P4.
-          assert (concatn eff1 eff 1 = eff1 ++ eff5).
-          { simpl_concatn. exact H21. }
-          rewrite H22 in P4. rewrite <- app_assoc in H19. pose (P5 := P4 _ H19).
-          inversion P5. inversion H23.
+          pose (P5 := P4 _ H15).
+          inversion P5. inversion H20.
 
     - intros. rewrite H4, H11 in *.
-      pose (EE2 := element_exist Value n kvals0 (eq_sym H12)).
-      pose (EE3 := element_exist Value n vvals0 (eq_sym H4)).
-      pose (EE4 := element_exist Value n0 kvals (eq_sym H5)).
-      pose (EE5 := element_exist Value n0 vvals (eq_sym H11)).
-      pose (EE6 := element_exist SideEffectList _ eff (eq_sym H7)).
-      pose (EE7 := element_exist SideEffectList _ eff7 (eq_sym H14)).
-      pose (EE8 := element_exist _ _ _ (eq_sym H8)).
-      pose (EE9 := element_exist _ _ _ (eq_sym H15)).
+      pose (EE2 := element_exist n kvals0 (eq_sym H12)).
+      pose (EE3 := element_exist n vvals0 (eq_sym H4)).
+      pose (EE4 := element_exist n0 kvals (eq_sym H5)).
+      pose (EE5 := element_exist n0 vvals (eq_sym H11)).
+      pose (EE6 := element_exist _ eff (eq_sym H7)).
+      pose (EE7 := element_exist _ eff7 (eq_sym H14)).
+      pose (EE8 := element_exist _ _ (eq_sym H8)).
+      pose (EE9 := element_exist _ _ (eq_sym H15)).
       inversion EE2 as [kv']. inversion EE3 as [vv']. inversion EE4 as [kv]. 
       inversion EE5 as [vv]. inversion EE6 as [e1]. inversion EE7 as [e1'].
       inversion EE8 as [id01]. inversion EE9 as [id01'].
       inversion H19. inversion H20. inversion H21. inversion H22.
       inversion H23. inversion H24. inversion H25. inversion H26. subst.
       inversion H7. inversion H14. inversion H8. inversion H15.
-      pose (EE10 := element_exist SideEffectList _ x3 (eq_sym H28)).
-      pose (EE11 := element_exist SideEffectList _ x4 (eq_sym H29)).
-      pose (EE12 := element_exist _ _ x5 (eq_sym H30)).
-      pose (EE13 := element_exist _ _ x6 (eq_sym H31)).
+      pose (EE10 := element_exist _ x3 (eq_sym H28)).
+      pose (EE11 := element_exist _ x4 (eq_sym H29)).
+      pose (EE12 := element_exist _ x5 (eq_sym H30)).
+      pose (EE13 := element_exist _ x6 (eq_sym H31)).
       inversion EE10 as [e2]. inversion EE11 as [e2'].
       inversion EE12 as [id02]. inversion EE13 as [id02'].
       inversion H27. inversion H32. inversion H33. inversion H34. subst.
@@ -1279,45 +1241,42 @@ Proof.
       (** FIRST ELEMENTS ARE EQUAL *)
       pose (F1 := H9 0 (Nat.lt_0_succ n)).
       pose (F2 := H 0 (Nat.lt_0_succ n0) _ _ _ F1). inversion F2. inversion H35.
-      destruct H36. simpl in H37.
-      simpl_concatn_app H36. simpl_concatn_H H36. apply app_inv_head in H36. subst.
+      destruct H36. simpl in H37, H36.
+      subst.
       pose (F3 := H10 0 (Nat.lt_0_succ n)).
       pose (F4 := H0 0 (Nat.lt_0_succ n0) _ _ _ F3). inversion F4. 
-      inversion H36. destruct H37. simpl in H38.
-      simpl_concatn_app H37. simpl_concatn_H H37. 
-      apply app_inv_head in H37. subst.
+      inversion H36. destruct H37. simpl in H38, H37. subst.
       (** OTHER ELEMETS *)
       assert (n0 = n /\ x1 = x /\ x2 = x0 /\ x7 = x8 /\ x9 = x10).
       {
-        eapply IHkl with (eff1 := eff1 ++ e1' ++ e2') (ex0 := ex0) (eff5 := eff5)
+        eapply IHkl with (* (eff1 := eff1 ++ e1' ++ e2') *) (ex0 := ex0) (eff5 := eff5)
              (eff4 := eff4) (eff2 := eff2) (val := val) (ex := ex) (vl := ves) (eff6 := eff6) (val0 := val0); auto.
         * intros. assert (S j < S n0). { omega. } pose (P3 := H (S j) H39 v2 eff''). simpl in P3.
-          rewrite concatn_app, concatn_app, concatn_app, Nat.add_0_r, <- plus_n_Sm, concatn_app,
-               <- app_assoc in P3. simpl in H38. rewrite Nat.add_0_r in H38.
+          simpl mult in H38, P3. rewrite Nat.add_0_r in H38, P3.
+          rewrite Nat.add_succ_r in P3. simpl in P3.
           pose (P4 := P3 _ H38). simpl. rewrite Nat.add_0_r. assumption.
         * intros. assert (S j < S n0). { omega. } pose (P3 := H0 (S j) H39 v2 eff''). simpl in P3.
-          rewrite concatn_app, concatn_app, concatn_app, Nat.add_0_r, <- plus_n_Sm, concatn_app,
-               <- app_assoc in P3. simpl in H38. rewrite Nat.add_0_r in H38.
+          simpl mult in H38, P3. rewrite Nat.add_0_r in H38, P3.
+          rewrite Nat.add_succ_r in P3. simpl in P3.
           pose (P4 := P3 _ H38). simpl. rewrite Nat.add_0_r. assumption.
         * intros. pose (P3 := H1 v2 eff'').
-          rewrite <- last_element_equal, <- last_element_equal in P3. simpl in P3.
-          rewrite concatn_app, Nat.add_0_r, <- plus_n_Sm, concatn_app, <- app_assoc in P3.
-          simpl. rewrite Nat.add_0_r. simpl in H37. rewrite Nat.add_0_r in H37.
+          rewrite <- last_element_equal, <- last_element_equal,
+                  <- last_element_equal, <- last_element_equal in P3. simpl in P3.
           apply (P3 _ H37).
         * intros. pose (P3 := H2 v2 eff''). simpl in P3.
-          rewrite concatn_app, Nat.add_0_r, <- plus_n_Sm, concatn_app, <- app_assoc in P3.
-          simpl in H37. rewrite Nat.add_0_r in H37. apply (P3 _ H37).
+          simpl in H37.
+          apply (P3 _ H37).
         * simpl in H6. omega.
         * intros. assert (S j < S n). { omega. } pose (P3 := H9 (S j) H38). simpl in P3.
-          rewrite concatn_app, concatn_app, concatn_app, Nat.add_0_r, <- plus_n_Sm, concatn_app,
-             <- app_assoc in P3. simpl. rewrite Nat.add_0_r. assumption.
+          rewrite Nat.add_succ_r in P3. simpl in P3.
+          simpl. rewrite Nat.add_0_r in *. assumption.
         * intros. assert (S j < S n). { omega. } pose (P3 := H10 (S j) H38). simpl in P3.
-          rewrite concatn_app, concatn_app, concatn_app, Nat.add_0_r, <- plus_n_Sm, concatn_app,
-             <- app_assoc in P3. simpl. rewrite Nat.add_0_r. assumption.
+          rewrite Nat.add_succ_r in P3. simpl in P3.
+          simpl. rewrite Nat.add_0_r in *. assumption.
         * simpl in H12. omega.
-        * rewrite <- last_element_equal, <- last_element_equal in H16. simpl in H16.
-          rewrite concatn_app, Nat.add_0_r, <- plus_n_Sm, concatn_app,
-                            <- app_assoc in H16. simpl. rewrite Nat.add_0_r. exact H16.
+        * rewrite <- last_element_equal, <- last_element_equal,
+                  <- last_element_equal, <- last_element_equal in H16. simpl in H16. 
+          exact H16.
       }
       destruct H37. destruct H38. destruct H39. destruct H40. subst. auto.
 Qed.
@@ -1330,32 +1289,32 @@ forall {vl : list Expression} (kvals vvals kvals0 vvals0 : list Value) (i : nat)
 (forall j : nat,
      j < i ->
      forall (v2 : Value + Exception) (eff'' : SideEffectList) (id'' : nat),
-     | env, nth_id ids id (2*j), nth j kl ErrorExp, concatn eff1 eff (2 * j) | -e>
+     | env, nth_def ids id 0 (2*j), nth j kl ErrorExp, nth_def eff eff1 [] (2 * j) | -e>
      | id'', v2, eff'' | ->
-     inl (nth j kvals ErrorValue) = v2 /\ concatn eff1 eff (S (2 * j)) = eff'' /\
-     nth_id ids id (S (2*j)) = id'')
+     inl (nth j kvals ErrorValue) = v2 /\ nth_def eff eff1 [] (S (2 * j)) = eff'' /\
+     nth_def ids id 0 (S (2*j)) = id'')
 ->
 (forall j : nat,
      j < i ->
      forall (v2 : Value + Exception) (eff'' : SideEffectList) (id'' : nat),
-     | env, nth_id ids id (S (2*j)), nth j vl ErrorExp, concatn eff1 eff (S (2 * j)) | -e>
+     | env, nth_def ids id 0 (S (2*j)), nth j vl ErrorExp, nth_def eff eff1 [] (S (2 * j)) | -e>
      | id'', v2, eff'' | ->
-     inl (nth j vvals ErrorValue) = v2 /\ concatn eff1 eff (S (S (2 * j))) = eff'' /\
-     nth_id ids id (S (S (2*j))) = id'')
+     inl (nth j vvals ErrorValue) = v2 /\ nth_def eff eff1 [] (S (S (2 * j))) = eff'' /\
+     nth_def ids id 0 (S (S (2*j))) = id'')
 ->
 (
 (forall (v2 : Value + Exception) (eff'' : SideEffectList) (id'' : nat),
-         | env, last ids id, nth i kl ErrorExp, concatn eff1 eff (2 * i) | -e>
+         | env, last ids id, nth i kl ErrorExp, last eff eff1 | -e>
          | id'', v2, eff'' | ->
-         inr ex = v2 /\ concatn eff1 eff (2 * i) ++ eff2 = eff'' /\ id1 = id'')
+         inr ex = v2 /\ eff2 = eff'' /\ id1 = id'')
 \/
 (forall (v2 : Value + Exception) (eff'' : SideEffectList) (id'' : nat),
-         | env, last ids id, nth i kl ErrorExp, concatn eff1 eff (2 * i) | -e>
+         | env, last ids id, nth i kl ErrorExp, last eff eff1 | -e>
          | id'', v2, eff'' | ->
-         inl val = v2 /\ concatn eff1 eff (2 * i) ++ eff2 = eff'' /\ id1 = id'')
+         inl val = v2 /\ eff2 = eff'' /\ id1 = id'')
 /\
 (forall (v2 : Value + Exception) (eff'' : SideEffectList) (id'' : nat),
-         | env, id1, nth i vl ErrorExp, concatn eff1 eff (2 * i) ++ eff2 | -e>
+         | env, id1, nth i vl ErrorExp, eff2 | -e>
          | id'', v2, eff'' | ->
          inr ex = v2 /\ eff4 = eff'' /\ id2 = id''))
 ->
@@ -1367,14 +1326,14 @@ Datatypes.length eff = (i * 2)%nat ->
 Datatypes.length ids = (i * 2)%nat ->
 (forall j : nat,
       j < length vl ->
-      | env, nth_id ids0 id (2*j), nth j kl ErrorExp, concatn eff1 eff7 (2 * j) | -e>
-      | nth_id ids0 id (S (2*j)), inl (nth j kvals0 ErrorValue),
-      concatn eff1 eff7 (S (2 * j)) |)
+      | env, nth_def ids0 id 0 (2*j), nth j kl ErrorExp, nth_def eff7 eff1 [] (2 * j) | -e>
+      | nth_def ids0 id 0 (S (2*j)), inl (nth j kvals0 ErrorValue),
+      nth_def eff7 eff1 [] (S (2 * j)) |)
 ->
 (forall j : nat,
   j < length vl ->
-  | env, nth_id ids0 id (S (2*j)), nth j vl ErrorExp, concatn eff1 eff7 (S (2 * j)) | -e>
-  | nth_id ids0 id (S (S (2*j))), inl (nth j vvals0 ErrorValue), concatn eff1 eff7 (S (S (2 * j))) |)
+  | env, nth_def ids0 id 0 (S (2*j)), nth j vl ErrorExp, nth_def eff7 eff1 [] (S (2 * j)) | -e>
+  | nth_def ids0 id 0 (S (S (2*j))), inl (nth j vvals0 ErrorValue), nth_def eff7 eff1 [] (S (S (2 * j))) |)
 ->
 length kl = Datatypes.length vvals0 ->
 length kl = Datatypes.length kvals0 ->
@@ -1398,7 +1357,7 @@ Proof.
     apply length_zero_iff_nil in H4.
     subst. auto.
   * intros. inversion H2.
-    pose (EE1 := element_exist Expression (length kl) vl H15).
+    pose (EE1 := element_exist (length kl) vl H15).
     inversion EE1 as [ve]. inversion H14 as [ves]. subst.
     case_eq (length vvals).
     - intros. apply length_zero_iff_nil in H3. subst. simpl length in *.
@@ -1412,17 +1371,17 @@ Proof.
       + pose (P1 := H3 _ _ _ E1). inversion P1. inversion H4.
       + inversion H3. pose (P1 := H4 _ _ _ E1). inversion P1. inversion H7. destruct H16.
         rewrite <- H16 in E2. subst.
-        pose (P2 := H6 _ _ _ E2). inversion P2. inversion H17.
+        pose (P2 := H6 _ _ _ E2). inversion P2. inversion H16.
 
     - intros. rewrite H3 in *.
-      pose (EE2 := element_exist Value _ kvals0 H11).
-      pose (EE3 := element_exist Value _ vvals0 H10).
-      pose (EE4 := element_exist Value _ kvals (eq_sym H4)).
-      pose (EE5 := element_exist Value _ vvals (eq_sym H3)).
-      pose (EE6 := element_exist SideEffectList _ eff (eq_sym H6)).
-      pose (EE7 := element_exist SideEffectList _ eff7 (eq_sym H12)).
-      pose (EE8 := element_exist nat _ _ (eq_sym H7)).
-      pose (EE9 := element_exist nat _ _ (eq_sym H13)).
+      pose (EE2 := element_exist _ kvals0 H11).
+      pose (EE3 := element_exist _ vvals0 H10).
+      pose (EE4 := element_exist _ kvals (eq_sym H4)).
+      pose (EE5 := element_exist _ vvals (eq_sym H3)).
+      pose (EE6 := element_exist _ eff (eq_sym H6)).
+      pose (EE7 := element_exist _ eff7 (eq_sym H12)).
+      pose (EE8 := element_exist _ _ (eq_sym H7)).
+      pose (EE9 := element_exist _ _ (eq_sym H13)).
       inversion EE2 as [kv']. inversion EE3 as [vv']. inversion EE4 as [kv]. 
       inversion EE5 as [vv]. inversion EE6 as [e1]. inversion EE7 as [e1']. 
       inversion EE8 as [id01]. inversion EE9 as [id01'].
@@ -1430,61 +1389,58 @@ Proof.
       inversion H20. inversion H21. inversion H22. inversion H23. subst.
 
       inversion H6. inversion H12. inversion H7. inversion H13.
-      pose (EE10 := element_exist SideEffectList _ _ (eq_sym H25)).
-      pose (EE11 := element_exist SideEffectList _ _ (eq_sym H26)).
-      pose (EE12 := element_exist _ _ _ (eq_sym H27)).
-      pose (EE13 := element_exist _ _ _ (eq_sym H28)).
+      pose (EE10 := element_exist _ _ (eq_sym H25)).
+      pose (EE11 := element_exist _ _ (eq_sym H26)).
+      pose (EE12 := element_exist _ _ (eq_sym H27)).
+      pose (EE13 := element_exist _ _ (eq_sym H28)).
       inversion EE10 as [e2]. inversion EE11 as [e2']. inversion EE12 as [id02].
       inversion EE13 as [id02'].
       inversion H24. inversion H29. inversion H30. inversion H31. subst.
       (** FIRST ELEMENTS ARE EQUAL *)
       pose (F1 := H8 0 (Nat.lt_0_succ (length ves))).
       pose (F2 := H 0 (Nat.lt_0_succ n) _ _ _ F1). inversion F2. inversion H32.
-      destruct H33. simpl in H34.
-      rewrite concatn_app, concatn_app in H33. simpl_concatn_H H33. apply app_inv_head in H33. subst.
+      destruct H33. simpl in H34, H33. subst.
       pose (F3 := H9 0 (Nat.lt_0_succ (length ves))).
       pose (F4 := H0 0 (Nat.lt_0_succ n) _ _ _ F3). inversion F4. inversion H33.
-      destruct H34. simpl in H35.
-      rewrite concatn_app, concatn_app in H34. simpl_concatn_H H34. apply app_inv_head in H34. subst.
+      destruct H34. simpl in H35, H34. subst.
       clear EE10. clear EE11. clear EE12. clear EE13.
       clear EE6. clear EE7. clear EE8. clear EE9. clear EE2. clear EE3.
       (** OTHER ELEMETS *)
       assert (n = length ves /\ x1 = x /\ x2 = x0 /\ x7 = x8 /\ x9 = x10).
       {
-        apply IHkl with (eff1 := eff1 ++ e1' ++ e2') (eff4 := eff4) (eff2 := eff2)
+        eapply IHkl with (* (eff1 := eff1 ++ e1' ++ e2') *) (eff4 := eff4) (eff2 := eff2)
                 (val := val) (ex := ex) (vl := ves) (id := id02') (id1 := id1) (id2 := id2); auto; clear IHkl.
         * intros. assert (S j < S n). { omega. }
-          pose (P3 := H (S j) H36 v2 eff''). simpl in P3.
-          rewrite concatn_app, concatn_app, concatn_app, Nat.add_0_r, <- plus_n_Sm, concatn_app,
-              <- app_assoc in P3. simpl in H35. rewrite Nat.add_0_r in H35.
+          pose (P3 := H (S j) H36 v2 eff'').
+          simpl mult in H35, P3. rewrite Nat.add_0_r in H35, P3.
+          rewrite Nat.add_succ_r in P3. simpl in P3.
           pose (P4 := P3 _ H35). simpl. rewrite Nat.add_0_r. assumption.
         * intros. assert (S j < S n). { omega. }
           pose (P3 := H0 (S j) H36 v2 eff''). simpl in P3.
-          rewrite concatn_app, concatn_app, concatn_app, Nat.add_0_r, <- plus_n_Sm, concatn_app,
-              <- app_assoc in P3. simpl in H35. rewrite Nat.add_0_r in H35.
+          simpl mult in H35, P3. rewrite Nat.add_0_r in H35, P3.
+          rewrite Nat.add_succ_r in P3. simpl in P3.
           pose (P4 := P3 _ H35). simpl. rewrite Nat.add_0_r. assumption.
         * intros. destruct H1 as [Def| Def'].
           - left. intros. simpl mult in Def, H1. simpl mult.
-          rewrite concatn_app, Nat.add_0_r, Nat.add_succ_r, concatn_app, <- app_assoc in Def.
-          rewrite Nat.add_0_r. rewrite Nat.add_0_r in H1. apply Def.
-            rewrite <- last_element_equal, <- last_element_equal. simpl. assumption.
+            apply Def.
+            repeat (rewrite <- last_element_equal). simpl. assumption.
           - right. simpl mult in Def'.
-            rewrite concatn_app, Nat.add_0_r, Nat.add_succ_r, concatn_app, <- app_assoc, 
+            rewrite <- last_element_equal, <- last_element_equal, 
                   <- last_element_equal, <- last_element_equal in Def'. simpl in Def'. inversion Def'.
             split.
-            + intros. simpl mult. rewrite Nat.add_0_r. apply H1. simpl mult in H35.
-              rewrite Nat.add_0_r in H35. assumption.
-            + intros. apply H34. simpl mult in H35. rewrite Nat.add_0_r in H35. assumption.
+            + intros. simpl mult. apply H1. simpl mult in H35.
+              assumption.
+            + intros. apply H34. simpl mult in H35. assumption.
 
         * simpl in H5. omega.
         * intros. assert (S j < S (length ves)). { omega. } pose (P3 := H8 (S j) H35).
           simpl in P3.
-          rewrite concatn_app, concatn_app, concatn_app, Nat.add_0_r, <- plus_n_Sm,
-             concatn_app, <- app_assoc in P3. simpl. rewrite Nat.add_0_r. assumption.
+          rewrite Nat.add_succ_r in P3. simpl in P3.
+          simpl. rewrite Nat.add_0_r in *. assumption.
         * intros. assert (S j < S (length ves)). { omega. }
           pose (P3 := H9 (S j) H35). simpl in P3. 
-          rewrite concatn_app, concatn_app, concatn_app, Nat.add_0_r, <- plus_n_Sm,
-               concatn_app, <- app_assoc in P3. simpl. rewrite Nat.add_0_r. assumption.
+          rewrite Nat.add_succ_r in P3. simpl in P3.
+          simpl. rewrite Nat.add_0_r in *. assumption.
       }
       destruct H34. destruct H35. destruct H36. destruct H37. subst. auto.
 Qed.
